Refactorings and cleanups in higher files: add PCUICContextConversion
Also change a lot of lemmas to use the == conversion relation instead of =

pcuic/theories/PCUICCumulativity.v
@@ -278,20 +278,61 @@ Hint Resolve red_conv_alt.
 
 Hint Resolve leq_term_refl cumul_refl' : core.
 
-Lemma conv_alt_red `{cf : checker_flags} :
-  forall Σ Γ t u,
-    Σ ;;; Γ |- t == u ->
-    ∑ t' u',
-      red Σ Γ t t' ×
-      red Σ Γ u u' ×
-      eq_term (global_ext_constraints Σ) t' u'.
+Lemma red_conv_conv `{cf : checker_flags} Σ Γ t u v :
+  red (fst Σ) Γ t u -> Σ ;;; Γ |- u == v -> Σ ;;; Γ |- t == v.
 Proof.
-  intros Σ Γ t u h. induction h.
-  - exists t, u. intuition auto.
-  - destruct IHh as [t' [u' [? [? ?]]]].
-    exists t', u'. intuition auto. now eapply red_step.
-  - destruct IHh as [t' [u' [? [? ?]]]].
-    exists t', u'. intuition auto. now eapply red_step.
+  intros. apply red_alt in X. apply clos_rt_rt1n_iff in X.
+  induction X; auto.
+  econstructor 2; eauto.
+Qed.
+
+Lemma red_conv_conv_inv `{cf : checker_flags} Σ Γ t u v :
+  red (fst Σ) Γ t u -> Σ ;;; Γ |- v == u -> Σ ;;; Γ |- v == t.
+Proof.
+  intros. apply red_alt in X. apply clos_rt_rt1n_iff in X.
+  induction X; auto.
+  now econstructor 3; [eapply IHX|]; eauto.
+Qed.
+
+Lemma conv_alt_sym `{cf : checker_flags} (Σ : global_env_ext) Γ t u :
+  wf Σ ->
+  Σ ;;; Γ |- t == u -> Σ ;;; Γ |- u == t.
+Proof.
+  intros wfΣ X.
+  induction X.
+  - eapply eq_term_sym in e; now constructor.
+  - eapply red_conv_conv_inv. eapply red1_red in r. eauto. eauto.
+  - eapply red_conv_conv. eapply red1_red in r. eauto. eauto.
+Qed.
+
+Lemma conv_alt_red {cf : checker_flags} {Σ : global_env_ext} {Γ : context} {t u : term} :
+  Σ;;; Γ |- t == u <~> (∑ v v' : term, (red Σ Γ t v × red Σ Γ u v') × eq_term (global_ext_constraints Σ) v v').
+Proof.
+  split. induction 1. exists t, u; intuition auto.
+  destruct IHX as [? [? [? ?]]].
+  exists x, x0; intuition auto. eapply red_step; eauto.
+  destruct IHX as [? [? [? ?]]].
+  exists x, x0; intuition auto. eapply red_step; eauto.
+  intros.
+  destruct X as [? [? [[? ?] ?]]].
+  eapply red_conv_conv; eauto.
+  eapply red_conv_conv_inv; eauto. now constructor.
+Qed.
+
+Lemma conv_alt_cumul `{cf : checker_flags} (Σ : global_env_ext) Γ t u : wf Σ ->
+  Σ ;;; Γ |- t == u -> Σ ;;; Γ |- t <= u.
+Proof.
+  intros wfΣ H.
+  apply conv_alt_red in H as [v [v' [[l r] eq]]].
+  apply cumul_alt.
+  exists v, v'; intuition auto. now eapply eq_term_leq_term.
+Qed.
+
+Lemma conv_alt_conv `{cf : checker_flags} (Σ : global_env_ext) Γ t u : wf Σ ->
+  Σ ;;; Γ |- t == u -> Σ ;;; Γ |- t = u.
+Proof.
+  intros wfΣ H. split. now apply conv_alt_cumul.
+  apply conv_alt_sym in H; auto. now apply conv_alt_cumul.
 Qed.
 
 Inductive conv_pb :=
@@ -300,28 +341,28 @@ Inductive conv_pb :=
 
 Definition conv `{cf : checker_flags} leq Σ Γ u v :=
   match leq with
-  | Conv => ∥ Σ ;;; Γ |- u = v ∥
+  | Conv => ∥ Σ ;;; Γ |- u == v ∥
   | Cumul => ∥ Σ ;;; Γ |- u <= v ∥
   end.
 
 Lemma conv_conv_l `{cf : checker_flags} :
-  forall Σ leq Γ u v,
-      Σ ;;; Γ |- u = v ->
+  forall (Σ : global_env_ext) leq Γ u v, wf Σ ->
+      Σ ;;; Γ |- u == v ->
       conv leq Σ Γ u v.
 Proof.
-  intros Σ [] Γ u v [h1 h2].
-  - cbn. constructor. constructor ; assumption.
+  intros Σ [] Γ u v h.
   - cbn. constructor. assumption.
+  - cbn. constructor. now apply conv_alt_cumul.
 Qed.
 
 Lemma conv_conv_r `{cf : checker_flags} :
-  forall Σ leq Γ u v,
-      Σ ;;; Γ |- u = v ->
+  forall (Σ : global_env_ext) leq Γ u v, wf Σ ->
+      Σ ;;; Γ |- u == v ->
       conv leq Σ Γ v u.
 Proof.
-  intros Σ [] Γ u v [h1 h2].
-  - cbn. constructor. constructor ; assumption.
-  - cbn. constructor. assumption.
+  intros Σ [] Γ u v wfΣ h.
+  - cbn. constructor. apply conv_alt_sym; auto.
+  - cbn. constructor. apply conv_alt_cumul. auto. now apply conv_alt_sym.
 Qed.
 
 Lemma cumul_App_l `{cf : checker_flags} :
