pcuic/theories/PCUICConversion.v
@@ -4,7 +4,8 @@ From Coq Require Import Bool String List Program BinPos Compare_dec Omega.
 From MetaCoq.Template Require Import config utils AstUtils.
 From MetaCoq.PCUIC Require Import PCUICAst PCUICAstUtils PCUICInduction
      PCUICLiftSubst PCUICUnivSubst PCUICTyping PCUICWeakeningEnv PCUICWeakening
-     PCUICReduction PCUICCumulativity PCUICConfluence PCUICParallelReductionConfluence PCUICEquality.
+     PCUICReduction PCUICCumulativity PCUICConfluence PCUICParallelReductionConfluence
+     PCUICEquality PCUICContextConversion.
 Require Import ssreflect ssrbool.
 Require Import String.
 From MetaCoq.Template Require Import LibHypsNaming.
@@ -17,103 +18,16 @@ Require Import Equations.Prop.DepElim.
 Ltac tc := try typeclasses eauto 10.
 Hint Resolve eq_universe_leq_universe : pcuic.
 
-Section RedEq.
-  Context {cf : checker_flags}.
-
-  Global Instance refl_eq_univ φ : Reflexive (eq_universe φ) := eq_universe_refl _.
-  Global Instance eq_univ_trans φ : Transitive (eq_universe φ) := eq_universe_trans _.
-  Global Instance refl_leq_univ φ : Reflexive (leq_universe φ) := leq_universe_refl _.
-  Global Instance leq_univ_trans φ : Transitive (leq_universe φ) := leq_universe_trans _.
-  Existing Class SubstUnivPreserving.
-  (* FIXME SubstUnivPreserving will need to be up-to a sigma or set of constraints at least *)
-  Global Instance eq_univ_substu φ : SubstUnivPreserving (eq_universe φ).
-  Admitted.
-  Global Instance leq_univ_substu φ : SubstUnivPreserving (leq_universe φ).
-  Admitted.
-
-  Context (Σ : global_env_ext).
-
-  Context {Re Rle} {refl : Reflexive Re} {refl' :Reflexive Rle} {sym : Symmetric Re}
-          {trre : Transitive Re} {trle : Transitive Rle} `{SubstUnivPreserving Re} `{SubstUnivPreserving Rle}.
-  Context (inclre : forall u u' : universe, Re u u' -> Rle u u').
-
-  Lemma red_eq_term_upto_univ_r {Γ T V U} :
-    eq_term_upto_univ Re Rle T U -> red Σ Γ U V ->
-    ∑ T', red Σ Γ T T' * eq_term_upto_univ Re Rle T' V.
-  Proof.
-    intros eq r.
-    apply red_alt in r.
-    induction r in T, eq |- *.
-    - eapply red1_eq_term_upto_univ_r in eq as [v' [r' eq']]; eauto.
-    - exists T; split; eauto.
-    - case: (IHr1 _ eq) => T' [r' eq'].
-      case: (IHr2 _ eq') => T'' [r'' eq''].
-      exists T''. split=>//.
-      now transitivity T'.
-  Qed.
-
-  Lemma red_eq_term_upto_univ_l {Γ u v u'} :
-    eq_term_upto_univ Re Rle u u' ->
-    red Σ Γ u v ->
-    ∑ v',
-    red Σ Γ u' v' *
-    eq_term_upto_univ Re Rle v v'.
-  Proof.
-    intros eq r.
-    eapply red_alt in r.
-    induction r in u', eq |- *.
-    - eapply red1_eq_term_upto_univ_l in eq as [v' [r' eq']]; eauto.
-    - exists u'. split; auto.
-    - case: (IHr1 _ eq) => T' [r' eq'].
-      case: (IHr2 _ eq') => T'' [r'' eq''].
-      exists T''. split=>//.
-      now transitivity T'.
-  Qed.
-
-  Lemma red_eq_term_upto_univ_lr {Γ l t u r} :
-    eq_term_upto_univ Re Rle l t -> eq_term_upto_univ Re Rle t r -> red Σ Γ t u ->
-    ∑ l' r', (red Σ Γ l l' * red Σ Γ r r') * eq_term_upto_univ Re Rle l' u * eq_term_upto_univ Re Rle u r'.
-  (* Proof. *)
-  (*   intros eq r. *)
-  (*   apply red_alt in r. *)
-  (*   induction r in T, eq |- *. *)
-  (*   - eapply red1_eq_term_upto_univ_r in eq as [v' [r' eq']]; eauto. *)
-  (*   - exists T; split; eauto. *)
-  (*   - case: (IHr1 _ eq) => T' [r' eq']. *)
-  (*     case: (IHr2 _ eq') => T'' [r'' eq'']. *)
-  (*     exists T''. split=>//. *)
-  (*     now transitivity T'. *)
-  (* Qed. *)
-  Admitted.
-  (* Lemma red_eq_term_upto_univ_back {Γ x y z} : *)
-  (*   red Σ Γ x y -> *)
-  (*   eq_term_upto_univ Re Rle y z -> *)
-  (*   ∑ x', *)
-  (*   red Σ Γ x' z * *)
-  (*   eq_term_upto_univ Re Rle x x. *)
-  (* Proof. *)
-  (*   intros eq r. *)
-  (*   eapply red_alt in r. *)
-  (*   induction r in u', eq |- *. *)
-  (*   - eapply red1_eq_term_upto_univ_l in eq as [v' [r' eq']]; eauto. *)
-  (*   - exists u'. split; auto. *)
-  (*   - case: (IHr1 _ eq) => T' [r' eq']. *)
-  (*     case: (IHr2 _ eq') => T'' [r'' eq'']. *)
-  (*     exists T''. split=>//. *)
-  (*     now transitivity T'. *)
-  (* Qed. *)
-
-End RedEq.
+Derive Signature for cumul assumption_context.
 
 Lemma congr_cumul_prod : forall `{checker_flags} Σ Γ na na' M1 M2 N1 N2,
-    Σ ;;; Γ |- M1 = N1 ->
+    Σ ;;; Γ |- M1 == N1 ->
     Σ ;;; (Γ ,, vass na M1) |- M2 <= N2 ->
     Σ ;;; Γ |- (tProd na M1 M2) <= (tProd na' N1 N2).
 Proof.
   intros.
 Admitted.
 
-Global Instance sym_eq_univ {cf : checker_flags} φ : Symmetric (eq_universe φ) := eq_universe_sym _.
 
 Lemma cumul_trans {cf:checker_flags} (Σ : global_env_ext) Γ t u v : wf Σ ->
   Σ ;;; Γ |- t <= u -> Σ ;;; Γ |- u <= v -> Σ ;;; Γ |- t <= v.
@@ -134,1442 +48,26 @@ Proof.
   eapply leq_term_trans with nf; eauto.
 Qed.
 
-Lemma red_conv_conv `{cf : checker_flags} Σ Γ t u v :
-  red (fst Σ) Γ t u -> Σ ;;; Γ |- u == v -> Σ ;;; Γ |- t == v.
+Lemma conv_trans {cf:checker_flags} (Σ : global_env_ext) Γ t u v : wf Σ ->
+  Σ ;;; Γ |- t = u -> Σ ;;; Γ |- u = v -> Σ ;;; Γ |- t = v.
 Proof.
-  intros. apply red_alt in X. apply clos_rt_rt1n_iff in X.
-  induction X; auto.
-  econstructor 2; eauto.
+  intros wfΣ tu uv.
+  split. eapply cumul_trans with u. auto. apply tu. apply uv.
+  eapply cumul_trans with u. auto. apply uv. apply tu.
 Qed.
 
-Lemma red_conv_conv_inv `{cf : checker_flags} Σ Γ t u v :
-  red (fst Σ) Γ t u -> Σ ;;; Γ |- v == u -> Σ ;;; Γ |- v == t.
+Lemma conv_sym {cf:checker_flags} (Σ : global_env_ext) Γ t u : wf Σ ->
+  Σ ;;; Γ |- t = u -> Σ ;;; Γ |- u = t.
 Proof.
-  intros. apply red_alt in X. apply clos_rt_rt1n_iff in X.
-  induction X; auto.
-  now econstructor 3; [eapply IHX|]; eauto.
+  intros wfΣ tu. split; apply tu.
 Qed.
 
-Lemma conv_alt_sym `{cf : checker_flags} (Σ : global_env_ext) Γ t u :
-  wf Σ ->
-  Σ ;;; Γ |- t == u -> Σ ;;; Γ |- u == t.
+(* Should follow from context conversion + invariants on T and U *)
+Lemma conv_conv_alt `{cf : checker_flags} {Σ : global_env_ext} (wfΣ : wf Σ) Γ T U :
+  Σ ;;; Γ |- T = U -> Σ ;;; Γ |- T == U.
 Proof.
-  intros wfΣ X.
-  induction X.
-  - eapply eq_term_sym in e; now constructor.
-  - eapply red_conv_conv_inv. eapply red1_red in r. eauto. eauto.
-  - eapply red_conv_conv. eapply red1_red in r. eauto. eauto.
-Qed.
-
-(* Lemma conv_conv_alt `{cf : checker_flags} (Σ : global_env_ext) Γ t u : wf Σ -> *)
-(*   Σ ;;; Γ |- t = u -> Σ ;;; Γ |- u == t. *)
-(* Proof. *)
-(*   intros wfΣ H. destruct H. *)
-(*   destruct H as (v & v' & (redv & redv') & leqv). *)
-(*   intros H'. apply cumul_alt in H'. *)
-(*   destruct H' as (v0 & v'0 & (redv0 & redv'0) & leqv0). *)
-(*   destruct (red_confluence wfΣ redv' redv0) as [nf [nfl nfr]]. *)
-(*   destruct (red_confluence wfΣ redv redv'0) as [nf' [nfl' nfr']]. *)
-(*   eapply red_eq_term_upto_univ_r in leqv; tc;eauto with pcuic. *)
-(*   destruct leqv as [v''0 [red'0 eq2]]. *)
-(*   eapply red_eq_term_upto_univ_l in leqv0; tc;eauto with pcuic. *)
-(*   destruct leqv0 as [v'1 [red'1 eq1]]. *)
-(*   eapply red_conv_conv; eauto. *)
-(*   eapply red_conv_conv; eauto. *)
-(*   eapply red_conv_conv_inv; eauto. *)
-(*   eapply red_conv_conv_inv; eauto. *)
-(*   eapply conv_sym; eauto. constructor. eapply eq_term_leq_term in eq1. *)
-
-Lemma conv_alt_red {cf : checker_flags} (Σ : global_env_ext) (Γ : context) (t u : term) :
-  Σ;;; Γ |- t == u <~> (∑ v v' : term, (red Σ Γ t v × red Σ Γ u v') × eq_term (global_ext_constraints Σ) v v').
-Proof.
-  split. induction 1. exists t, u; intuition auto.
-  destruct IHX as [? [? [? ?]]].
-  exists x, x0; intuition auto. eapply red_step; eauto.
-  destruct IHX as [? [? [? ?]]].
-  exists x, x0; intuition auto. eapply red_step; eauto.
-  intros.
-  destruct X as [? [? [[? ?] ?]]].
-  eapply red_conv_conv; eauto.
-  eapply red_conv_conv_inv; eauto. now constructor.
-Qed.
-
-(* Needs context conversion too *)
-(* Lemma congr_cumul_prod : forall `{checker_flags} Σ Γ na na' M1 M2 N1 N2, *)
-(*   conv Σ Γ M1 N1 -> *)
-(*   cumul Σ (Γ ,, vass na M1) M2 N2 -> *)
-(*   cumul Σ Γ (tProd na M1 M2) (tProd na' N1 N2). *)
-(* Proof. *)
-(*   intros. *)
-(* Admitted. *)
-
-Lemma leq_term_antisym `{cf : checker_flags} (Σ : constraints) t u :
-  leq_term Σ t u -> leq_term Σ u t -> eq_term Σ t u.
 Admitted.
 
-(* Lemma leq_term_antisym' `{cf : checker_flags} (Σ : constraints) t u t' Γ : *)
-(*   leq_term Σ t u -> leq_term Σ u t' -> *)
-(*   joinable (red Σ Γ) t t' -> *)
-(*   eq_term Σ t u * eq_term Σ t' u. *)
-(* Admitted. *)
-
-Coercion global_ext_constraints : global_env_ext >-> constraints.
-
-Require Import PCUICParallelReduction PCUICParallelReductionConfluence.
-
-Lemma cumul_trans_red `{cf : checker_flags} {Σ : global_env_ext} {Γ t u v} : wf Σ ->
-  Σ ;;; Γ |- t <= u -> Σ ;;; Γ |- u <= v ->
-  ∑ l o r, red Σ Γ t l *
-           red Σ Γ u o *
-           red Σ Γ v r *
-           leq_term Σ l o * leq_term Σ o r.
-Proof.
-  intros wfΣ X X0.
-  eapply cumul_alt in X as [v' [v'' [[redl redr] eq]]].
-  eapply cumul_alt in X0 as [w [w' [[redl' redr'] eq']]].
-  destruct (red_confluence wfΣ redr redl') as [nf [nfl nfr]].
-  eapply red_eq_term_upto_univ_r in eq; tc;eauto with pcuic.
-  destruct eq as [v'0 [red'0 eq2]].
-  eapply red_eq_term_upto_univ_l in eq'; tc;eauto with pcuic.
-  destruct eq' as [v'1 [red'1 eq1]].
-  exists v'0, nf, v'1.
-  repeat split.
-  transitivity v'; auto.
-  transitivity w; auto.
-  transitivity w'; auto.
-  eapply leq_term_trans with nf; eauto.
-  eapply leq_term_trans with nf; eauto.
-Qed.
-
-Unset Universe Minimization ToSet.
-Lemma clos_rt_eq_term `{cf : checker_flags} {Σ : global_env_ext} :
-  inclusion (clos_refl_trans (eq_term Σ)) (eq_term Σ).
-Proof.
-  intros x y. induction 1. auto. apply eq_term_refl. now apply eq_term_trans with y.
-Qed.
-
-Lemma clos_rt_eq_leq_term `{cf : checker_flags} {Σ : global_env_ext} :
-  inclusion (clos_refl_trans (eq_term Σ)) (leq_term Σ).
-Proof.
-  intros x y. induction 1. auto. apply eq_term_leq_term. now apply eq_term_trans with y. apply leq_term_refl.
-  now apply leq_term_trans with y.
-Qed.
-
-Lemma clos_rt_leq_term `{cf : checker_flags} {Σ : global_env_ext} :
-  inclusion (clos_refl_trans (leq_term Σ)) (leq_term Σ).
-Proof.
-  intros x y. induction 1. auto. apply leq_term_refl. now apply leq_term_trans with y.
-Qed.
-
-Lemma leq_term_upto_univ_confluent `{cf : checker_flags} {Σ : global_env_ext} :
-  diamond (eq_term Σ).
-Proof.
-  intros x y. intros.
-  exists x. split. now apply eq_term_sym. now apply eq_term_sym.
-Qed.
-
-Lemma All_All2_All2_mix {A B} (P : B -> B -> Type) (Q R : A -> B -> Type) l l' l'' :
-  All (fun x => forall y z, Q x y -> R x z -> ∑ v, P y v * P z v) l -> All2 Q l l' -> All2 R l l'' ->
-  ∑ l''', All2 P l' l''' * All2 P l'' l'''.
-Proof.
-  intros H; induction H in l', l'' |- *;
-  intros H' H''; depelim H'; depelim H''; try solve [econstructor; eauto; constructor].
-  simpl. destruct (IHAll _ _ H' H''). destruct (p _ _ q r).
-  exists (x1 :: x0). split; constructor; intuition auto.
-Qed.
-
-(* Lemma All_All2_All2_mix_hetero {A B} (P : B -> B -> Type) (Q R : A -> B -> Type) l l' l'' : *)
-(*   All (fun x => forall y z, Q x y -> R x z -> ∑ v, P y v * P z v) l -> All2 Q l l' -> All2 R l l'' -> *)
-(*   ∑ l''', All2 P l' l''' * All2 P l'' l'''. *)
-(* Proof. *)
-(*   intros H; induction H in l', l'' |- *; *)
-(*   intros H' H''; depelim H'; depelim H''; try solve [econstructor; eauto; constructor]. *)
-(*   simpl. destruct (IHAll _ _ H' H''). destruct (p _ _ q r). *)
-(*   exists (x1 :: x0). split; constructor; intuition auto. *)
-(* Qed. *)
-
-Lemma eq_term_upto_univ_incl `{cf:checker_flags} Re Rle : inclusion Re Rle -> inclusion (eq_term_upto_univ Re Re)
-                                                                    (eq_term_upto_univ Re Rle).
-Proof. intros. intros x y H. eapply eq_term_upto_univ_leq in H; eauto. Qed.
-
-Set Implicit Arguments.
-Unset Strict Implicit.
-
-Lemma All_inst {A : Type} {C : Type} {l : list C} {P : A -> C -> Type} :
-  All (fun x : C => forall a : A, P a x) l -> forall x : A, All (P x) l.
-Proof.
-  intros. eapply All_impl; eauto.
-Qed.
-
-Hint Extern 10 => solve [reflexivity] : core.
-
-Local Tactic Notation "join" uconstr(x) := exists x; intuition (constructor; eauto).
-
-Lemma diamond_All2_diamond {A} (R : relation A) : diamond R -> diamond (All2 R).
-Proof.
-  intros HR l l' l'' Hl Hl'.
-  induction Hl in l'', Hl' |- ; depelim Hl'.
-  join [].
-  destruct (IHHl _ Hl') as [tl' [? ?]].
-  destruct (HR _ _ _ r r0) as [hd' [? ?]].
-  join (hd' :: tl').
-Qed.
-
-Definition first_level (u : universe) :=
-  match u with
-  | NEL.sing a => fst a
-  | NEL.cons a _ => fst a
-  end.
-
-Lemma make_first_level : forall l, first_level (Universe.make l) = l.
-Proof. by case. Qed.
-
-(* Lemma first_level_make : forall l, Universe.make (first_level u) = l. *)
-(* Proof. by case. Qed. *)
-
-Lemma diamond_map {A B} (R : relation A) (f : B -> A) (g : A -> B) :
-  (forall x, x = f (g x)) ->
-  diamond R -> diamond (on_Trel R f).
-Proof.
-  intros Hf HR l l' l'' Hl Hl'. red in Hl, Hl'.
-  destruct (HR _ _ _ Hl Hl') as [hd' [? ?]].
-  rewrite (Hf hd') in r, r0.
-  join (g hd').
-Qed.
-
-Lemma All2_impl_hetero {A B C D : Type} (P : A -> B -> Type) (Q : C -> D -> Type) l l' (f : A -> C) (g : B -> D) :
-  (forall x y, P x y -> Q (f x) (g y)) ->
-  All2 P l l' ->
-  All2 (fun x y => Q (f x) (g y)) l l'.
-Proof.
-  intros HP. induction 1; constructor; auto.
-Qed.
-
-(* Lemma All_impl_hetero {A B C D : Type} (P : A -> B -> Type) (Q : C -> D -> Type) l l' (f : A -> C) (g : B -> D) : *)
-(*   (forall x y, P x y -> Q (f x) (g y)) -> *)
-(*   All P l -> *)
-(*   All2 (fun x y => Q (f x) (g y)) l l'. *)
-(* Proof. *)
-(*   intros HP. induction 1; constructor; auto. *)
-(* Qed. *)
-
-Definition diamond_on {A} (R : A -> A -> Type) (x : A) := forall y z, R x y -> R x z -> joinable R y z.
-
-Lemma eq_term_upto_univ_diamomd :
-  forall (Re Rle : universe -> universe -> Type),
-    inclusion Re Rle ->
-    diamond Re ->
-    diamond Rle ->
-    diamond (eq_term_upto_univ Re Rle).
-Proof.
-  intros Re Rle Rincl hRe hRle x.
-  fold (diamond_on (eq_term_upto_univ Re Rle) x).
-  induction x in Re, Rle, Rincl, hRe, hRle |- * using term_forall_list_ind;
-    intros y z eq eq'.
-  all: dependent destruction eq; dependent destruction eq'.
-  all: try solve [ eexists; split; constructor ].
-  Ltac t := intuition (constructor; eauto).
-
-  - do 2 eapply All_inst with Re in X.
-    do 3 eapply All_inst in X; eauto.
-    eapply All_All2_All2_mix in X; [|eapply a|eapply a0].
-    destruct X as [nf [H H']]. exists (tEvar n nf).
-    split; constructor; auto.
-
-  - destruct (hRle _ _ _ e e0).
-    join (tSort x).
-
-  - specialize (IHx1 Re Re ltac:(eauto) hRe hRe _ _ eq1 eq'1) as [dom [? ?]].
-    specialize (IHx2 Re _ ltac:(eauto) hRe hRle _ _ eq2 eq'2) as [codom [? ?]].
-    join (tProd na' dom codom).
-
-  - specialize (IHx1 Re Re ltac:(eauto) hRe hRe _ _ eq1 eq'1) as [dom [? ?]].
-    specialize (IHx2 Re _ ltac:(eauto) hRe hRle _ _ eq2 eq'2) as [codom [? ?]].
-    join (tLambda na' dom codom).
-
-  - specialize (IHx1 Re Re ltac:(eauto) hRe hRe _ _ eq1 eq'1) as [def [? ?]].
-    specialize (IHx2 Re Re ltac:(eauto) hRe hRe _ _ eq2 eq'2) as [ty [? ?]].
-    specialize (IHx3 Re _ ltac:(eauto) hRe hRle _ _ eq3 eq'3) as [body [? ?]].
-    join (tLetIn na' def ty body).
-
-  - specialize (IHx1 Re _ ltac:(eauto) hRe hRle _ _ eq1 eq'1) as [fn [? ?]].
-    specialize (IHx2 Re Re ltac:(eauto) hRe hRe _ _ eq2 eq'2) as [arg [? ?]].
-    join (tApp fn arg).
-
-  - eapply diamond_All2_diamond in hRle.
-    destruct (hRle _ _ _ a a0) as [u'' ?].
-    (* eexists (tConst s (map first_level u'')); t. *)
-    (* This is wrong: we need specific Rie Rile relations for comparision
-       of universes instances which are levels only *)
-    todo "universe instances".
-
-  - todo "universe instances".
-  - todo "universe instances".
-
-  - specialize (IHx1 Re Re ltac:(eauto) hRe hRe _ _ eq1 eq'1) as [fn [? ?]].
-    specialize (IHx2 Re Re ltac:(eauto) hRe hRe _ _ eq2 eq'2) as [arg [? ?]].
-    red in X.
-    do 2 eapply All_inst with Re in X. do 3 eapply All_inst in X; eauto.
-
-    eapply (All_impl (Q:=fun x => diamond_on (relation_conjunction (on_Trel eq fst)
-                                                                   (on_Trel (eq_term_upto_univ Re Re) snd)) x)) in X.
-    2:{ rewrite /diamond_on /= //.
-        move=> [an t] H [ax ty] [az tz].
-        rewrite /on_Trel => /= [] /= [] /= -> eq3 [] /= -> eq4.
-        destruct (H ty tz eq3 eq4).
-        join (az, x) => /=. }
-    eapply All_All2_All2_mix in X as [brs [? ?]].
-    2:{ eapply All2_impl. eapply a. t. }
-    2:{ eapply All2_impl. eapply a0. t. }
-    join (tCase (ind, par) fn arg brs) => //.
-
-  - specialize (IHx Re Re ltac:(eauto) hRe hRe _ _ eq eq') as [arg [? ?]].
-    join (tProj s arg).
-
-  - red in X.
-    eapply (All_impl (Q:=fun x =>
-                           diamond_on (fun x y =>
-                                         (eq_term_upto_univ Re Re (dtype x) (dtype y)) *
-                                         (eq_term_upto_univ Re Re (dbody x) (dbody y)) *
-                                         (rarg x = rarg y)) x))%type in X.
-    2:{ rewrite /diamond_on /= //.
-        move=> [na ty' body' arg'] /= [Hty Hbod] y z.
-        move=> [[]] eqty eqbod -> [[]] eqty' eqbod' eq.
-        destruct (Hty _ Re ltac:(eauto) hRe hRe _ _ eqty eqty') as [dtype [? ?]].
-        destruct (Hbod _ Re ltac:(eauto) hRe hRe _ _ eqbod eqbod') as [dbody [? ?]].
-        join {| dname := dname y; dtype := dtype; dbody := dbody; rarg := rarg z |} => /=. }
-    eapply All_All2_All2_mix in X as [mfix [? ?]]; cycle 1.
-    eapply All2_impl; [eapply a|]; intuition auto; intuition auto.
-    eapply All2_impl; [eapply a0|]; intuition auto; intuition auto.
-    join (tFix mfix n) => //.
-
-  - red in X.
-    eapply (All_impl (Q:=fun x =>
-                           diamond_on (fun x y =>
-                                         (eq_term_upto_univ Re Re (dtype x) (dtype y)) *
-                                         (eq_term_upto_univ Re Re (dbody x) (dbody y)) *
-                                         (rarg x = rarg y)) x))%type in X.
-    2:{ rewrite /diamond_on /= //.
-        move=> [na ty' body' arg'] /= [Hty Hbod] y z.
-        move=> [[]] eqty eqbod -> [[]] eqty' eqbod' eq.
-        destruct (Hty _ Re ltac:(eauto) hRe hRe _ _ eqty eqty') as [dtype [? ?]].
-        destruct (Hbod _ Re ltac:(eauto) hRe hRe _ _ eqbod eqbod') as [dbody [? ?]].
-        join {| dname := dname y; dtype := dtype; dbody := dbody; rarg := rarg z |} => /=. }
-    eapply All_All2_All2_mix in X as [mfix [? ?]]; cycle 1.
-    eapply All2_impl; [eapply a|]; intuition auto; intuition auto.
-    eapply All2_impl; [eapply a0|]; intuition auto; intuition auto.
-    join (tCoFix mfix n) => //.
-Qed.
-
-Lemma leq_universe_sup_l `{cf : checker_flags} u v φ : leq_universe φ u (Universe.sup u v).
-  todo "Universes specification".
-Admitted.
-
-Lemma leq_universe_sup_r `{cf : checker_flags} u v φ : leq_universe φ v (Universe.sup u v).
-  todo "Universes specification".
-Admitted.
-
-Lemma eq_term_upto_univ_diamond `{cf : checker_flags} {Σ : global_env_ext} :
-  diamond (eq_term Σ).
-Proof.
-  eapply eq_term_upto_univ_diamomd. firstorder.
-  red. intros x y z eq eq'. exists x. split; auto using eq_universe_sym.
-  red. intros x y z eq eq'. exists x. split; auto using eq_universe_sym.
-Qed.
-
-Lemma leq_term_upto_univ_diamond `{cf : checker_flags} {Σ : global_env_ext} :
-  diamond (leq_term Σ).
-Proof.
-  (* This corresponds to the fact that for universes `l, u, v`,
-     if `l <= u` /\ `l <= v` then `u <= max(u, v)` `v <= max(u, v)` *)
-  eapply eq_term_upto_univ_diamomd. apply: (eq_universe_leq_universe _).
-  red. intros x y z eq eq'. exists x. split; auto using eq_universe_sym.
-  red. intros x y z eq eq'. exists (Universe.sup y z).
-  split; auto using leq_universe_sup_l, leq_universe_sup_r.
-Qed.
-
-Lemma commutes_eqterm_red1 {cf : checker_flags} {Σ : global_env_ext} Γ : commutes (eq_term Σ) (red1 Σ Γ).
-Proof.
-  intros x y z.
-  intros.
-  eapply red1_eq_term_upto_univ_l in H; tc; eauto.
-Qed.
-
-Lemma commutes_leqterm_red1 {cf : checker_flags} {Σ : global_env_ext} Γ : commutes (leq_term Σ) (red1 Σ Γ).
-Proof.
-  intros x y z.
-  intros.
-  eapply red1_eq_term_upto_univ_l in H; tc; eauto. intros. now eapply eq_universe_leq_universe.
-Qed.
-
-Generalizable Variables A B R S T.
-
-Definition rel_cart {A B} (R : relation A) (S : relation B) : relation (A * B) :=
-  fun x y => (R x.1 y.1 * S x.2 y.2)%type.
-Hint Unfold rel_cart : core.
-
-Instance rel_cart_refl `{HR : Reflexive A R} `{HS : Reflexive B T} :
-  Reflexive (rel_cart R T).
-Proof. auto. Qed.
-
-Instance rel_cart_trans `{HR : Transitive A R} `{HS : Transitive B T} :
-  Transitive (rel_cart R T).
-Proof. firstorder auto. Qed.
-
-Instance rel_cart_sym `{HR : Symmetric A R} `{HS : Symmetric B T} :
-  Symmetric (rel_cart R T).
-Proof. firstorder auto. Qed.
-
-Definition leq_term_rel {cf : checker_flags} Σ : relation (context * term) :=
-  rel_cart eq (leq_term Σ).
-
-Definition eq_term_rel {cf : checker_flags} Σ : relation (context * term) :=
-  rel_cart eq (eq_term Σ).
-
-Lemma commutes_leqterm_pred1 {cf : checker_flags} {Σ : global_env_ext} :
-  commutes (@pred1_rel Σ) (leq_term_rel Σ).
-Proof.
-  intros x y z.
-  intros.
-  (* eapply red1_eq_term_upto_univ_l in H; tc; eauto. intros. now eapply eq_universe_leq_universe. *)
-Admitted.
-
-Lemma commutes_eqterm_pred1 {cf : checker_flags} {Σ : global_env_ext} :
-  commutes (@pred1_rel Σ) (eq_term_rel Σ).
-Proof.
-  intros x y z.
-  intros.
-  (* eapply red1_eq_term_upto_univ_l in H; tc; eauto. intros. now eapply eq_universe_leq_universe. *)
-Admitted.
-
-Definition red1_or_leq {cf : checker_flags} (Σ : global_env_ext) (Γ : context) :=
-  relation_disjunction (leq_term Σ) (red1 Σ Γ).
-
-Definition red1_leq {cf : checker_flags} (Σ : global_env_ext) : relation (context * term) :=
-  relation_disjunction (@red1_rel_alpha Σ) (leq_term_rel Σ).
-
-Definition red1_eq {cf : checker_flags} (Σ : global_env_ext) : relation (context * term) :=
-  relation_disjunction (@red1_rel_alpha Σ) (eq_term_rel Σ).
-
-Definition pred1_leq {cf : checker_flags} (Σ : global_env_ext) :=
-  relation_disjunction (@pred1_rel Σ) (leq_term_rel Σ).
-
-Definition pred1_eq {cf : checker_flags} (Σ : global_env_ext) :=
-  relation_disjunction (@pred1_rel Σ) (eq_term_rel Σ).
-
-Instance leq_term_refl {cf : checker_flags} Σ : Reflexive (leq_term Σ).
-Proof. intros x; apply leq_term_refl. Defined.
-
-Instance leq_term_trans {cf : checker_flags} Σ : Transitive (leq_term Σ).
-Proof. intros x; apply leq_term_trans. Defined.
-
-Instance eq_term_refl {cf : checker_flags} Σ : Reflexive (eq_term Σ).
-Proof. intros x; apply eq_term_refl. Defined.
-
-Instance eq_term_trans {cf : checker_flags} Σ : Transitive (eq_term Σ).
-Proof. intros x; apply eq_term_trans. Defined.
-
-Lemma pred1_leq_confluence {cf : checker_flags} (Σ : global_env_ext) : wf Σ -> confluent (pred1_leq Σ).
-Proof.
-  intros wfΣ.
-  apply confluent_union. tc. intros x. red. apply pred1_refl.
-  apply commutes_leqterm_pred1. apply (diamond_pred1_rel wfΣ).
-  move=> [Γ x] [Δ y] [Ψ z] [] /= -> leqxy [] /= -> leqyz.
-  destruct (leq_term_upto_univ_diamond leqxy leqyz) as [nf [redl redr]].
-  exists (Ψ, nf); firstorder.
-Qed.
-
-Lemma pred1_eq_confluence {cf : checker_flags} (Σ : global_env_ext) : wf Σ -> confluent (pred1_eq Σ).
-Proof.
-  intros wfΣ.
-  apply confluent_union. tc. intros x. red. apply pred1_refl.
-  apply commutes_eqterm_pred1. apply (diamond_pred1_rel wfΣ).
-  move=> [Γ x] [Δ y] [Ψ z] [] /= -> leqxy [] /= -> leqyz.
-  destruct (eq_term_upto_univ_diamond leqxy leqyz) as [nf [redl redr]].
-  exists (Ψ, nf); firstorder.
-Qed.
-
-Hint Unfold leq_term_rel : core.
-
-Lemma red1_leq_confluence {cf : checker_flags} (Σ : global_env_ext) : wf Σ -> confluent (red1_leq Σ).
-Proof.
-  intros wfΣ.
-  notypeclasses refine (fst (sandwich _ _ _ _) _).
-  3:eapply pred1_leq_confluence; eauto.
-  intros [ctx t] [ctx' t'].
-  rewrite /red1_leq /pred1_leq /=.
-  move=> [l|[/= <- r]].
-  - left. now eapply red1_rel_alpha_pred1_rel.
-  - right. auto.
-  - intros [Γ x] [Δ y] [l|r].
-    eapply clos_rt_disjunction_left.
-    now apply pred1_rel_red1_rel_alpha.
-    eapply clos_rt_disjunction_right.
-    now constructor.
-Qed.
-
-Lemma red1_eq_confluence {cf : checker_flags} (Σ : global_env_ext) : wf Σ -> confluent (red1_eq Σ).
-Proof.
-  intros wfΣ.
-  notypeclasses refine (fst (sandwich _ _ _ _) _).
-  3:eapply pred1_eq_confluence; eauto.
-  intros [ctx t] [ctx' t'].
-  rewrite /red1_leq /pred1_leq /=.
-  move=> [l|[/= <- r]].
-  - left. now eapply red1_rel_alpha_pred1_rel.
-  - right. red; auto.
-  - intros [Γ x] [Δ y] [l|r].
-    eapply clos_rt_disjunction_left.
-    now apply pred1_rel_red1_rel_alpha.
-    eapply clos_rt_disjunction_right.
-    now constructor.
-Qed.
-
-Lemma red1_incl_red1_leq {cf : checker_flags} (Σ : global_env_ext) Γ :
-  wf Σ -> forall x y, red Σ Γ x y -> clos_refl_trans (red1_leq Σ) (Γ, x) (Γ, y).
-Proof.
-  intros wfΣ.
-  intros x y rxy.
-  eapply red_alt in rxy.
-  induction rxy. constructor. red. left. left. split; auto.
-  constructor 2.
-  now transitivity (Γ, y).
-Qed.
-
-Lemma leq_incl_red1_leq {cf : checker_flags} (Σ : global_env_ext) Γ :
-  wf Σ -> forall x y, leq_term Σ x y -> clos_refl_trans (red1_leq Σ) (Γ, x) (Γ, y).
-Proof.
-  intros wfΣ.
-  intros x y rxy. constructor. right. red; auto.
-Qed.
-
-Lemma cumul_trans_red_eqterm `{cf : checker_flags} {Σ : global_env_ext} {Γ t u v} : wf Σ ->
-  Σ ;;; Γ |- t <= u -> Σ ;;; Γ |- u <= v ->
-  ∑ l o r, red Σ Γ t l *
-           red Σ Γ u o *
-           red Σ Γ v r *
-           leq_term Σ l o * leq_term Σ o r.
-Proof.
-  intros wfΣ X X0.
-  intros.
-  eapply cumul_alt in X as [t0 [u0 [[redl redr] eq]]].
-  eapply cumul_alt in X0 as [u1 [v0 [[redl' redr'] eq']]].
-  destruct (red_confluence wfΣ redr redl') as [unf [nfl nfr]].
-  eapply red_eq_term_upto_univ_r in eq; tc;eauto with pcuic.
-  destruct eq as [t1 [red'0 eq2]].
-  eapply red_eq_term_upto_univ_l in eq'; tc;eauto with pcuic.
-  destruct eq' as [v1 [red'1 eq1]].
-  exists t1, unf, v1.
-  repeat split.
-  transitivity t0; auto.
-  transitivity u0; auto.
-  transitivity v0; auto. eapply eq2. eapply eq1.
-Qed.
-
-Definition rel_comp {A} (R S : relation A) :=
-  fun x z => ∑ y, R x y * S y z.
-
-Lemma commutes_clos_rt_one {A} (R S : relation A) :
-  commutes R S -> commutes (clos_refl_trans R) S.
-Proof.
-  intros Hcom x y z Hxy Hxz.
-  eapply clos_rt_rt1n_iff in Hxy.
-  induction Hxy in z, Hxz |- *.
-  - exists z. split; auto.
-  - destruct (Hcom _ _ _ r Hxz) as [j [jl jr]].
-    specialize (IHHxy _ jl).
-    destruct IHHxy as [w [szw Rjw]].
-    exists w. split; auto. transitivity j => //. now constructor.
-Qed.
-
-Lemma commutes_sym {A} (R S : relation A) :
-  commutes R S -> commutes S R.
-Proof.
-  intros Hcom x y z Hxy Hxz.
-  destruct (Hcom _ _ _ Hxz Hxy) as [j [jl jr]].
-  exists j. split; auto.
-Qed.
-
-Lemma commutes_clos_rt {A} (R S : relation A) :
-  commutes R S -> commutes (clos_refl_trans R) (clos_refl_trans S).
-Proof.
-  intros. apply commutes_clos_rt_one.
-  eapply commutes_sym. eapply commutes_clos_rt_one.
-  now eapply commutes_sym.
-Qed.
-
-(* Lemma clos_rt_disjunction_mon {A} (R S : relation A) : *)
-(*   relation_equivalence (clos_refl_trans (relation_disjunction R S)) *)
-(*                        (relation_disjunction (clos_refl_trans R) (clos_refl_trans S)). *)
-(* Proof. *)
-(*   split. *)
-(*   induction 1. *)
-(*   destruct r. *)
-(*   - left. now constructor. *)
-(*   - right; now constructor. *)
-(*   - left. now constructor 2. *)
-(*   - destruct IHX1. *)
-
-Definition commutes_horizontal {A} (R S : relation A) :=
-  inclusion (rel_comp R S) (rel_comp S R).
-
-Lemma commutes_horizontal_red_leq {cf : checker_flags} (Σ : global_env_ext) Γ :
-  commutes_horizontal (leq_term Σ) (red Σ Γ).
-Proof.
-  intros x z. move=> [y [Hl Hr]].
-  red.
-  eapply red_eq_term_upto_univ_r in Hl. all:tc. 3:eapply Hr.
-  2:eapply (eq_universe_leq_universe _).
-  eapply Hl.
-Qed.
-
-Lemma commutes_horizontal_leq_red1_alpha_rels {cf : checker_flags} {Σ : global_env_ext} :
-  commutes_horizontal (leq_term_rel Σ) (@red1_rel_alpha Σ).
-Proof.
-  intros [Γ x] [Δ z]. move=> [[Ψ y] [[/= -> Hl] Hr]].
-  destruct Hr as [Hr|[Hr|Hr]].
-  - destruct Hr as [Hr ->].
-    eapply red1_eq_term_upto_univ_r in Hl as [mid [rmid leqmid]]. all:tc.
-    3:eapply Hr.
-    2:eapply eq_universe_leq_universe.
-    exists (Δ, mid). split; firstorder.
-  - destruct Hr as [Hr ->].
-    exists (Δ, x). split; firstorder auto.
-  - destruct Hr as [Hr ->].
-    exists (Δ, x). split; firstorder auto.
-Qed.
-
-Hint Resolve rt_refl rt_step : core.
-
-Lemma commutes_horizontal_clos_rt_right {A} (R S : relation A) :
-  commutes_horizontal R S ->
-  commutes_horizontal R (clos_refl_trans S).
-Proof.
-  intros HRS.
-  intros x z [y [Hl Hr]].
-  apply clos_rt_rt1n_iff in Hr.
-  induction Hr in x, Hl |- *.
-  - exists x. split; auto.
-  - destruct (HRS x y) as [mid [Smid Rmid]]. exists x0; auto.
-    destruct (IHHr _ Rmid) as [mid' [Smid' Rmid']].
-    exists mid'; intuition auto.
-    now eapply rt_trans with mid.
-Qed.
-
-Lemma commutes_horizontal_clos_rt {A} (R S : relation A) :
-  commutes_horizontal R S ->
-  commutes_horizontal (clos_refl_trans R) (clos_refl_trans S).
-Proof.
-  intros HRS.
-  eapply commutes_horizontal_clos_rt_right.
-  intros x z [y [Hl Hr]].
-  eapply clos_rt_rtn1_iff in Hl.
-  induction Hl in z, Hr.
-  - now exists z.
-  - destruct (HRS y z) as [mid [Smid Rmid]].
-    now exists z0.
-    destruct (IHHl _ Smid) as [mid' [Smid' Rmid']].
-    exists mid'; intuition auto.
-    now eapply rt_trans with mid.
-Qed.
-
-Lemma commutes_horizontal_clos_rt_disj {A} (R S : relation A) :
-  commutes_horizontal S R ->
-  inclusion (clos_refl_trans (relation_disjunction R S))
-            (rel_comp (clos_refl_trans R) (clos_refl_trans S)).
-Proof.
-  intros Hcom x y Hxy.
-  (* eapply commutes_clos_rt in Hcom. *)
-  eapply clos_rt_rt1n_iff in Hxy.
-  induction Hxy.
-  - exists x. split. now constructor 2. now constructor 2.
-  - destruct IHHxy as [y' [yy' y'z]].
-    destruct r.
-    * exists y'. split; auto.
-      eapply clos_rt_rt1n_iff. eapply rt1n_trans. eauto. now eapply clos_rt_rt1n_iff.
-    * eapply commutes_horizontal_clos_rt_right in Hcom.
-      destruct (Hcom x y') as [mid [Rmid Smid]].
-      now exists y.
-      exists mid; intuition auto.
-      now eapply rt_trans with y'.
-Qed.
-
-Lemma clos_rt_refl_trans {A} {R : relation A} `{Reflexive A R} `{Transitive A R} :
-  relation_equivalence (clos_refl_trans R) R.
-Proof.
-  split.
-  induction 1; auto. now transitivity y.
-  intros. auto.
-Qed.
-
-Definition red_leq {cf : checker_flags} Σ Γ := fun x y => clos_refl_trans (red1_leq Σ) (Γ, x) (Γ, y).
-
-Instance red_leq_trans {cf : checker_flags} (Σ : global_env_ext) Γ :
-  Transitive (red_leq Σ Γ).
-Proof. unfold red_leq. intros x y z Hxy Hyz. now transitivity (Γ, y). Qed.
-
-Definition red_comp_leq `{cf : checker_flags} (Σ : global_env_ext) Γ t u :=
-  ∑ t', red Σ Γ t t' * leq_term Σ t' u.
-
-Lemma clos_rt_red1_leq_spec `{cf : checker_flags} {Σ : global_env_ext} {t u} :
-  wf Σ -> clos_refl_trans (red1_leq Σ) t u -> red_comp_leq Σ t.1 t.2 u.2.
-Proof.
-  intros.
-  eapply commutes_horizontal_clos_rt_disj in X0 as [[Δ mid] [r leq]].
-  exists mid.
-  split; auto. eapply clos_rt_red1_alpha_out in r as [Hctx Ht]=>//. simpl in *.
-  - now eapply red_alt.
-  - unshelve eapply (fst (clos_rt_refl_trans _ _)) in leq; tc.
-    red in leq. red in leq. simpl in leq. intuition auto.
-  - eapply commutes_horizontal_leq_red1_alpha_rels.
-Qed.
-
-Lemma red_leq_spec `{cf : checker_flags} {Σ : global_env_ext} {Γ t u} :
-  wf Σ -> red_leq Σ Γ t u <~> red_comp_leq Σ Γ t u.
-Proof.
-  intros. split.
-  - intros X0; eapply commutes_horizontal_clos_rt_disj in X0 as [[Δ mid] [r leq]].
-    exists mid.
-    split; auto. eapply clos_rt_red1_alpha_out in r as [Hctx Ht]=>//. simpl in *.
-    * now eapply red_alt.
-    * unshelve eapply (fst (clos_rt_refl_trans _ _)) in leq; tc.
-      red in leq. red in leq. simpl in leq. intuition auto.
-    * eapply commutes_horizontal_leq_red1_alpha_rels.
-
-  - intros X0. destruct X0 as [v [redtv leqvu]].
-    eapply rt_trans with (Γ, v).
-    eapply clos_rt_disjunction_left.
-    now eapply clos_rt_red1_red1_rel_alpha, red_alt.
-    eapply clos_rt_disjunction_right.
-    constructor. auto.
-Qed.
-
-(* Lemma cumul_alt_red_leq `{cf : checker_flags} {Σ : global_env_ext} {Γ t u} : *)
-(*    wf Σ -> *)
-(*    Σ ;;; Γ |- t <= u -> *)
-(*    ∑ o o', red Σ Γ t o * *)
-(*            leq_term Σ o o' * *)
-(*            red Σ Γ u o'. *)
-(* Proof. *)
-(*   intros. *)
-(*   eapply cumul_alt in X0 as [v [v' [[redl redr] leq]]]. *)
-(*   exists v'. split; red; auto. *)
-(*   - transitivity (Γ, v). apply clos_rt_disjunction_left. *)
-(*     eapply red_alt in redl. now apply clos_rt_red1_red1_rel_alpha. *)
-(*     constructor. right. red; auto. *)
-(*   - eapply clos_rt_disjunction_left. *)
-(*     apply red_alt in redr. now eapply clos_rt_red1_red1_rel_alpha. *)
-(* Qed. *)
-
-Lemma confluence_clos_rt_red1_leq `{cf : checker_flags} {Σ : global_env_ext} {Γ t u v} :
-  wf Σ ->
-  clos_refl_trans (red1_leq Σ) (Γ, t) (Γ, u) ->
-  clos_refl_trans (red1_leq Σ) (Γ, t) (Γ, v) ->
-  ∑ nf, red_leq Σ Γ u nf * red_leq Σ Γ v nf.
-Proof.
-  intros wfΣ tu tv.
-  destruct (red1_leq_confluence wfΣ tu tv) as [[Δ nf] [redl redr]].
-  exists nf; auto.
-  eapply clos_rt_red1_leq_spec in redl=>//.
-  eapply clos_rt_red1_leq_spec in redr=>//.
-  simpl in *.
-  split; now eapply red_leq_spec.
-Qed.
-
-Lemma commutes_eqterm_red {cf : checker_flags} {Σ : global_env_ext} {Γ} : commutes (eq_term Σ) (clos_refl_trans (red1 Σ Γ)).
-Proof.
-  eapply commutes_sym, commutes_clos_rt_one, commutes_sym.
-  eapply commutes_eqterm_red1.
-Qed.
-
-Lemma commutes_leqterm_red {cf : checker_flags} {Σ : global_env_ext} {Γ} : commutes (leq_term Σ) (clos_refl_trans (red1 Σ Γ)).
-Proof.
-  eapply commutes_sym, commutes_clos_rt_one, commutes_sym.
-  eapply commutes_leqterm_red1.
-Qed.
-
-(* Lemma commutes_leqterm_red' {cf : checker_flags} {Σ : global_env_ext} {Γ} : commutes (leq_term Σ) (red Σ Γ). *)
-(* Proof. *)
-(*   eapply commutes_sym. *)
-(*   apply commutes_proper. *)
-(*  commutes_clos_rt_one, commutes_sym. *)
-(*   eapply commutes_leqterm_red1. *)
-(* Qed. *)
-
-Lemma cumul_trans_red_leqterm `{cf : checker_flags} {Σ : global_env_ext} {Γ t u v} : wf Σ ->
-  Σ ;;; Γ |- t <= u -> Σ ;;; Γ |- u <= v ->
-  ∑ o mid o', red Σ Γ t o *
-       leq_term Σ o mid *
-       red Σ Γ u mid *
-       leq_term Σ mid o' *
-       red Σ Γ v o'.
-Proof.
-  intros wfΣ X X0.
-  intros.
-  eapply cumul_alt in X as [t' [u' [[ol or] leq]]] => //.
-  eapply cumul_alt in X0 as [u'' [v' [[o'l o'r] leq']]] => //.
-  destruct (red_confluence wfΣ or o'l) as [unf [tl rr]].
-  assert (∑ tnf, red Σ Γ t' tnf * leq_term Σ tnf unf).
-  apply commutes_horizontal_red_leq. exists u'; auto.
-  destruct X as [tnf [ttnf tnfunf]].
-  destruct (commutes_leqterm_red leq' (equiv _ _ (red_alt Σ _ _ _) rr)) as [v'nf [? ?]].
-  eapply red_alt in c.
-  exists tnf, unf, v'nf.
-  intuition auto. now transitivity t'.
-  now transitivity u''.
-  now transitivity v'.
-Qed.
-
-(* Lemma cumul_trans_red_leqterm' `{cf : checker_flags} {Σ : global_env_ext} {Γ t u} : wf Σ -> *)
-(*   Σ ;;; Γ |- t <= u -> Σ ;;; Γ |- u <= t -> *)
-(*   ∑ o mid, red Σ Γ t o * *)
-(*        leq_term Σ o mid * *)
-(*        red Σ Γ u mid * *)
-(*        leq_term Σ mid o. *)
-(* Proof. *)
-(*   intros wfΣ X X0. *)
-(*   intros. *)
-(*   eapply cumul_alt in X as [t' [u' [[ol or] leq]]] => //. *)
-(*   eapply cumul_alt in X0 as [u'' [v' [[o'l o'r] leq']]] => //. *)
-
-(*   Lemma confluence_uniqueness `{cf : checker_flags} {Σ : global_env_ext} {Γ t u} : *)
-(*     wf Σ -> *)
-(*     red Σ Γ t t' -> *)
-(*     red Σ Γ t t'' -> *)
-(*     ∑ tnf, red Σ Γ t' tnf * red Σ Γ t'' tnf. *)
-
-
-(*   destruct (red_confluence wfΣ or o'l) as [unf [ul ur]]. *)
-(*   destruct (red_confluence wfΣ ol o'r) as [tnf [tl rr]]. *)
-(*   assert (leq_term Σ tnf unf). *)
-(*   split; auto. *)
-(*   eapply red_eq_term_upto_univ_l in tl. 9:eapply leq. all:tc. 2:eapply eq_universe_leq_universe. *)
-(*   destruct tl as [tnf' [rnf' leqnf']]. transitivity tnf'. auto. *)
-(*   eapply red_eq_term_upto_univ_r in rr. 10:eapply leq'. all:tc. 2:eapply eq_universe_leq_universe. *)
-(*   destruct rr as [tnf'' [rnf'' leqnf'']]. transitivity tnf''. auto. *)
-
-
-
-(*   apply commutes_horizontal_red_leq. exists u'; auto. *)
-(*   destruct X as [tnf' [ttnf tnfunf]]. *)
-(*   destruct (commutes_leqterm_red leq' (equiv _ _ (red_alt Σ _ _ _) ur)) as [v'nf [? ?]]. *)
-(*   eapply red_alt in c. *)
-(*   exists tnf, unf. *)
-(*   intuition auto. now transitivity t'. *)
-(*   now transitivity u''. *)
-(*   now transitivity v'. *)
-(* Qed. *)
-
-(* Lemma cumul_trans_red_leq `{cf : checker_flags} {Σ : global_env_ext} {Γ t u v} : wf Σ -> *)
-(*   Σ ;;; Γ |- t <= u -> Σ ;;; Γ |- u <= v -> *)
-(*   ∑ mid, red_leq Σ Γ t mid * *)
-(*          red Σ Γ u mid * *)
-(*          red_geq Σ Γ v mid. *)
-(*          red_leq Σ Γ u o' * *)
-(*        red Σ Γ u mid * *)
-(*        leq_term Σ mid o' * *)
-(*        red Σ Γ v o'. *)
-(* Proof. *)
-(*   intros wfΣ X X0. *)
-(*   intros. *)
-(*   eapply cumul_alt in X as [t' [u' [[ol or] leq]]] => //. *)
-(*   eapply cumul_alt in X0 as [u'' [v' [[o'l o'r] leq']]] => //. *)
-(*   destruct (red_confluence wfΣ or o'l) as [unf [tl rr]]. *)
-(*   assert (∑ tnf, red Σ Γ t' tnf * leq_term Σ tnf unf). *)
-(*   apply commutes_horizontal_red_leq. exists u'; auto. *)
-(*   destruct X as [tnf [ttnf tnfunf]]. *)
-(*   destruct (commutes_leqterm_red leq' (equiv _ _ (red_alt Σ _ _ _) rr)) as [v'nf [? ?]]. *)
-(*   eapply red_alt in c. *)
-(*   exists tnf, unf, v'nf. *)
-(*   intuition auto. now transitivity t'. *)
-(*   now transitivity u''. *)
-(*   now transitivity v'. *)
-(* Qed. *)
-
-Lemma red_red_leq `{cf : checker_flags} {Σ : global_env_ext} {Γ} t u :
-  wf Σ ->
-  red Σ Γ t u -> red_leq Σ Γ t u.
-Proof.
-  intros wfΣ tu. eapply red_alt in tu.
-  red. induction tu; try solve [econstructor; eauto].
-  constructor. red. left. left. auto.
-Qed.
-
-Lemma leq_red_leq `{cf : checker_flags} {Σ : global_env_ext} {Γ} t u :
-  wf Σ ->
-  leq_term Σ t u -> red_leq Σ Γ t u.
-Proof.
-  intros wfΣ tu.
-  red.
-  constructor. red. right. red; auto.
-Qed.
-
-Lemma cumul_trans_red_conv_aux `{cf : checker_flags} {Σ : global_env_ext} {Γ t u} : wf Σ ->
-  Σ ;;; Γ |- t <= u -> Σ ;;; Γ |- u <= t ->
-  (∃ v : term, red_leq Σ Γ t v × red Σ Γ u v).
-Proof.
-  intros wfΣ X X0.
-  eapply cumul_alt in X as [v [v' [[tv uv'] leq]]].
-  eapply cumul_alt in X0 as [w [w' [[tw uw'] leq']]].
-  destruct (red_confluence wfΣ uv' tw) as [tj [? ?]].
-  exists tj. intuition auto.
-  - transitivity v; auto. now apply red_red_leq.
-    transitivity v'. now eapply leq_red_leq.
-    now eapply red_red_leq.
-  - transitivity v'; auto.
-Qed.
-
-Lemma cumul_conv_lr {cf : checker_flags} {Σ : global_env_ext} {Γ t u t' u'} :
-  wf Σ ->
-  Σ ;;; Γ |- t = t' ->
-  Σ ;;; Γ |- u = u' ->
-  Σ ;;; Γ |- t <= u ->
-  Σ ;;; Γ |- t' <= u'.
-Proof.
-  intros.
-  destruct X0, X1.
-  eapply cumul_trans with u; auto.
-  eapply cumul_trans with t; auto.
-Qed.
-
-Lemma conv_conv_alt `{cf : checker_flags} {Σ : global_env_ext} {wfΣ : wf Σ} Γ t u :
-  Σ ;;; Γ |- t == u -> Σ ;;; Γ |- t = u.
-Proof.
-  induction 1.
-  constructor; constructor. now eapply eq_term_leq_term.
-  eapply eq_term_leq_term; now apply eq_term_sym.
-  constructor. econstructor 2; eauto. apply IHX.
-  econstructor 3. 2:eauto. apply IHX.
-  constructor. econstructor 3. 2:eauto. apply IHX.
-  econstructor 2; eauto. apply IHX.
-Qed.
-
-Lemma cumul_conv'_lr {cf : checker_flags} {Σ : global_env_ext} {Γ t u t' u'} :
-  wf Σ ->
-  Σ ;;; Γ |- t == t' ->
-  Σ ;;; Γ |- u == u' ->
-  Σ ;;; Γ |- t <= u ->
-  Σ ;;; Γ |- t' <= u'.
-Proof.
-  intros.
-  eauto using cumul_conv_lr, conv_conv_alt.
-Qed.
-
-(*
-   t0  <=  u0
-   |       |
-   |       |
-   v       v
-   t' >=   u
-   |       |
-   |       |
-   t'' <= u''
-*)
-
-Lemma fill_le `{cf : checker_flags} {Σ : global_env_ext} {Γ t t' u u'} :
-  wf Σ ->
-  leq_term Σ t u -> red Σ Γ t t' -> red Σ Γ u u' ->
-  ∑ t'' u'', red Σ Γ t' t'' * red Σ Γ u' u'' * leq_term Σ t'' u''.
-Proof.
-  intros wfΣ tu tt' uu'.
-  pose proof tu as tu2.
-  eapply red_eq_term_upto_univ_l in tu. 9:eapply tt'. all:tc. 2:eapply eq_universe_leq_universe.
-  destruct tu as [u'' [uu'' t'u'']].
-  destruct (red_confluence wfΣ uu' uu'') as [unf [ul ur]].
-  eapply red_eq_term_upto_univ_r in t'u''. 10:eapply ur. all:tc. 2:eapply eq_universe_leq_universe.
-  destruct t'u'' as [t'' [t't'' t''unf]].
-  exists t'', unf. intuition auto.
-Qed.
-
-Instance eq_term_sym@{i j} {cf : checker_flags} φ :
-  Symmetric@{i j} (eq_term_upto_univ (eq_universe φ) (eq_universe φ)) | (Symmetric (eq_term_upto_univ _ _)).
-Proof.
-  apply eq_term_upto_univ_sym.
-  intros x y; eapply eq_universe_sym.
-Qed.
-
-Hint Unfold eq_term : typeclass_instances.
-
-Instance leq_refl@{i j} (Re Rle : crelation@{i j} _) :
-  Reflexive Re -> Reflexive Rle -> Reflexive@{i j} (eq_term_upto_univ Re Rle).
-Proof. intros ** x. now apply eq_term_upto_univ_refl. Qed.
-
-Instance leq_trans@{i j} (Re Rle : crelation@{i j} _) :
-  Transitive Re -> Transitive Rle -> Transitive@{i j} (eq_term_upto_univ Re Rle).
-Proof. intros ** x. now apply eq_term_upto_univ_trans. Qed.
-
-Instance incl Re Rle :
-  inclusion Re Rle -> inclusion (eq_term_upto_univ Re Re) (eq_term_upto_univ Re Rle).
-Proof. intros H x y. eapply eq_term_upto_univ_leq. auto. Qed.
-
-Lemma eq_context_upto_nth_error Re Γ Γ' n :
-  Reflexive Re ->
-  eq_context_upto Re Γ Γ' ->
-  match nth_error Γ n with
-  | Some d => ∑ d', (nth_error Γ' n = Some d') * eq_decl_upto Re d d'
-  | None => nth_error Γ' n = None
-  end.
-Proof.
-  intros Rerefl.
-  induction Γ in Γ', n |- *.
-  - move=> H. depelim H =>//. now rewrite nth_error_nil.
-  - case: n => //=.
-    * move=> H. depelim H.
-      eexists; intuition eauto. constructor; simpl; auto. constructor.
-      eexists; intuition eauto. constructor; simpl; auto.
-      constructor; simpl; auto.
-    * move=> n eqc. depelim eqc.
-      eapply IHΓ; eauto.
-      eapply IHΓ; eauto.
-Qed.
-
-Section RhoLeqTerm.
-
-  (* Lemma pred1_preserves_eq_Term (Σ : global_env) Γ Δ Δ' t t' t'' *)
-  (*       {Re Rle} {refl : Equivalence Re} {refl' :Reflexive Rle} *)
-  (*       {Rleanti : Antisymmetric Re Rle} *)
-  (*       {trle : Transitive Rle} `{SubstUnivPreserving Re} `{SubstUnivPreserving Rle} *)
-  (*       {inclre : inclusion Re Rle}: *)
-  (*   pred1 Σ Γ Δ t t' -> *)
-  (*   pred1 Σ Γ Δ' t t'' -> *)
-  (*   eq_term_upto_univ Re Rle t' t'' -> *)
-  (*   eq_term_upto_univ Re Re t' t''. *)
-  (* Proof. *)
-  (*   intros Hs. *)
-  (*   set(P' := *)
-  (*         fun (Γl Γr : context) => True). *)
-  (*           (* eq_context_upto Re Γl Γr). *) *)
-  (*   intros Ht Hu. revert Γ Δ t t' Hs Δ' t'' Ht Hu. *)
-  (*   refine (pred1_ind_all_ctx Σ _ P' _ _ _ _ _ _ _ _ _ _ _ _ _ _ _ _ _ _ _ _ _ _); intros *; !intros; subst P'; *)
-  (*     simpl in *. *)
-
-  (*   - auto. *)
-
-  (*   - depelim Ht. as *)
-  (*     apply eq_term_upto_univ_subst; auto. *)
-  (*     eapply (forall_Δ' (Δ' ,, vass na t3)). assumption. eauto. admit. *)
-
-
-(*   Lemma pred1_preserves_eq_Term (Σ : global_env) Γ Δ Δ' t u t' u' *)
-(*         {Re Rle} {refl : Equivalence Re} {refl' :Reflexive Rle} *)
-(*         {Rleanti : Antisymmetric Re Rle} *)
-(*         {trle : Transitive Rle} `{SubstUnivPreserving Re} `{SubstUnivPreserving Rle} *)
-(*         {inclre : inclusion Re Rle}: *)
-(*     eq_term_upto_univ Re Rle t u -> *)
-(*     pred1 Σ Γ Δ t t' -> *)
-(*     pred1 Σ Γ Δ' u u' -> *)
-(*     eq_term_upto_univ Re (flip Rle) t' u' -> *)
-(*     eq_term_upto_univ Re Rle t' u'. *)
-(*   Proof. *)
-(*     intros Hs. *)
-(*     set(P' := *)
-(*           fun (Γl Γr : context) => True). *)
-(*             (* eq_context_upto Re Γl Γr). *) *)
-(*     intros Ht Hu. revert Γ Δ t t' Ht Δ' u Hs u' Hu. *)
-(*     refine (pred1_ind_all_ctx Σ _ P' _ _ _ _ _ _ _ _ _ _ _ _ _ _ _ _ _ _ _ _ _ _); intros *; !intros; subst P'; *)
-(*       simpl in *. *)
-
-(*     - auto. *)
-
-(*     - depelim Hs. depelim Hu. depelim Hs1. *)
-(*       apply eq_term_upto_univ_subst; auto. *)
-(*       eapply (forall_Δ' (Δ' ,, vass na0 t3)); eauto. admit. *)
-(* s *)
-
-
-  (*     try subst Γ Γ'; simplify_IH_hyps; cbn -[iota_red]; *)
-  (*     match goal with *)
-  (*       |- context [iota_red _ _ _ _] => idtac *)
-  (*     | |- _ => autorewrite with lift *)
-  (*     end; *)
-  (*     try specialize (forall_Γ _ _ _ eq_refl _ _ _ *)
-  (*                              _ _ Hs eq_refl heq_length heq_length0 HΔ); *)
-  (*   try specialize (forall_Γ0 _ _ _ eq_refl _ _ _ *)
-  (*                             _ _ Hs eq_refl heq_length heq_length0 HΔ); *)
-  (*   try specialize (forall_Γ1 _ _ _ eq_refl _ _ _ *)
-  (*                          _ _ Hs eq_refl heq_length heq_length0 HΔ); *)
-  (*     try pose proof (All2_local_env_length X0); *)
-  (*     simpl; try solve [ econstructor; eauto; try apply All2_map; *)
-  (*                        unfold All2_prop_eq, All2_prop, on_Trel, id in *; solve_all]; *)
-  (*       unfold All2_prop_eq, All2_prop, on_Trel, id in *. *)
-
-  (*   set(P' := *)
-  (*         fun (Γl Γr : context) => *)
-  (*           forall (Γ Δ : context) (Γ' : list context_decl), *)
-  (*             Γl = Γ ,,, Δ ,,, Γ' -> *)
-  (*             forall (Γ1 : list context_decl) (Δ1 : context) (Γ'1 : list context_decl) (s s' : list term), *)
-  (*               psubst Σ Γ Γ1 s s' Δ Δ1 -> *)
-  (*               Γr = Γ1 ,,, Δ1 ,,, Γ'1 -> *)
-  (*               #|Γ| = #|Γ1| -> *)
-  (*              All2_local_env_over (pred1 Σ) Γ Γ1 Δ Δ1 -> *)
-  (*              pred1_ctx Σ (Γ ,,, subst_context s 0 Γ') (Γ1 ,,, subst_context s' 0 Γ'1)). *)
-  (*   refine (pred1_ind_all_ctx Σ _ P' _ _ _ _ _ _ _ _ _ _ _ _ _ _ _ _ _ _ _ _ _ _); intros *; !intros; *)
-  (*     try subst Γ Γ'; simplify_IH_hyps; cbn -[iota_red]; *)
-  (*     match goal with *)
-  (*       |- context [iota_red _ _ _ _] => idtac *)
-  (*     | |- _ => autorewrite with lift *)
-  (*     end; *)
-
-
-  (* Definition same_shape Σ Γ Δ (x y z w : term) (rl : pred1 Σ Γ Δ x y) (rr : pred1 Σ Γ Δ z w) : Type := *)
-  (*   True. *)
-
-  (* Lemma red_confluence_upto {cf : checker_flags} {Σ : global_env_ext} {Γ Δ t l r} : *)
-  (*   pred1 Σ Γ Δ t l -> pred1 Σ Γ Δ t r -> *)
-  (*   leq_term Σ l r -> *)
-  (*   ∑ t' (rl : pred1 Σ Γ Δ l t') (rr : pred1 Σ Γ Δ r t'), same_shape rl rr. *)
-  (* Proof. *)
-  (*   intros. *)
-  (*   destruct (confluence *)
-
-
-  (*   move=> H H'. apply red_alt in H. apply red_alt in H'. *)
-  (*   destruct (red1_confluent wfΣ _ _ _ _ H H') as [nf [redl redr]]. *)
-  (*   apply red_alt in redl; apply red_alt in redr. *)
-  (*   exists nf; intuition auto. *)
-  (* Qed. *)
-
-
-
-  (* Lemma rho_leq_term {Σ : global_env_ext} *)
-  (*       {Re Rle} {refl : Equivalence Re} {refl' :Reflexive Rle} *)
-  (*       {Rleanti : Antisymmetric Re Rle} *)
-  (*       {trle : Transitive Rle} `{SubstUnivPreserving Re} `{SubstUnivPreserving Rle} *)
-  (*       {inclre : inclusion Re Rle} Γ Γ' t u : *)
-  (*   eq_term_upto_univ Re Rle t u -> *)
-  (*   eq_context_upto Re (rho_ctx Σ Γ) (rho_ctx Σ Γ') -> *)
-  (*   (* eq_term_upto_univ Re (flip Rle) (rho Σ (rho_ctx Σ Γ) t) (rho Σ (rho_ctx Σ Γ') u) -> *) *)
-  (*   eq_term_upto_univ Re Rle (rho Σ (rho_ctx Σ Γ) t) (rho Σ (rho_ctx Σ Γ') u). *)
-  (* Proof. *)
-  (*   intros eqt eqctx. *)
-  (*   move t before Σ. move Γ before t. move Γ' before Γ. move eqctx before Γ'. move u before t. *)
-  (*   move eqt before u. *)
-  (*   induction t using term_forall_list_ind in u, Re, Rle, eqt, Γ, Γ', eqctx, *)
-  (*                                             refl, refl', trle, inclre |- *; depelim eqt. *)
-  (*   all:cbn;try (constructor; auto). *)
-  (*   all:solve_all. *)
-  (*   - generalize (eq_context_upto_nth_error n _ eqctx). *)
-  (*     case: (nth_error (rho_ctx Σ Γ) n) => //=. *)
-  (*     move => [na [b|] ty] /= [d' [-> eqd]]; depelim eqd; simpl in *. *)
-  (*     depelim r. rewrite H. apply lift_eq_term_upto_univ. eapply incl; auto. *)
-  (*     depelim r. rewrite H. reflexivity. *)
-  (*     move=> -> /=. reflexivity. *)
-
-  (*   - specialize (IHt2 _ Re Rle eqt2 (Γ ,, vass n t1) (Γ' ,, vass na' a')). *)
-  (*     simpl in IHt2. rewrite !app_context_nil_l in IHt2. *)
-  (*     eapply IHt2; auto. constructor. eapply IHt1; auto. *)
-  (*     auto. *)
-
-  (*   - specialize (IHt2 _ Re Rle eqt2 (Γ ,, vass n t1) (Γ' ,, vass na' ty')). *)
-  (*     simpl in IHt2. rewrite !app_context_nil_l in IHt2. *)
-  (*     eapply IHt2; auto. constructor. eapply IHt1; auto. *)
-  (*     auto. *)
-
-  (*   - specialize (IHt3 _ Re Rle eqt3 (Γ ,, vdef n t1 t2) (Γ' ,, vdef na' t' ty')). *)
-  (*     simpl in IHt3. rewrite !app_context_nil_l in IHt3. *)
-  (*     transitivity (((rho Σ (vdef na' (rho Σ (rho_ctx Σ Γ') t') (rho Σ (rho_ctx Σ Γ') ty') :: rho_ctx Σ Γ') u') {0 *)
-  (*    := rho Σ (rho_ctx Σ Γ) t1})). eapply PCUICSubstitution.subst_eq_term_upto_univ. auto. auto. *)
-  (*     eapply IHt3; auto. constructor. eapply IHt1; auto. *)
-  (*     auto. auto. *)
-  (* Admitted. *)
-
-  (* Lemma red_confluence_upto {cf : checker_flags} {Σ : global_env_ext} {Γ t t' u v} : *)
-  (*   leq_term Σ t t' -> *)
-  (*   red Σ Γ t u -> red Σ Γ t' v -> *)
-
-  (*   ∑ v' v'', red Σ Γ u v' * red Σ Γ v v'' * leq_term Σ v' v''. *)
-  (* Proof. *)
-  (* Admitted. *)
-  (*   move=> H H'. apply red_alt in H. apply red_alt in H'. *)
-  (*   destruct (red1_confluent wfΣ _ _ _ _ H H') as [nf [redl redr]]. *)
-  (*   apply red_alt in redl; apply red_alt in redr. *)
-  (*   exists nf; intuition auto. *)
-  (* Qed. *)
-End RhoLeqTerm.
-
-
-(* Lemma red_leq_same `{cf : checker_flags} {Σ : global_env_ext} {Γ x y} : *)
-(*   wf Σ -> *)
-(*   red1 Σ Γ x y -> leq_term Σ y x -> False. *)
-(* Proof. *)
-(*   intros wfΣ xy yx. *)
-(*   induction y in Γ, x, xy, yx |- * using term_forall_list_ind. *)
-(*   all: depelim yx; try solve [depelim xy; solve_discr]. *)
-(*   Ltac t' := firstorder eauto using eq_term_leq_term. *)
-(*   - depelim xy. admit. *)
-(*     solve_discr. *)
-(*   - depelim xy; solve_discr. *)
-(*     admit. *)
-(*   - depelim xy; solve_discr; t'. *)
-(*   - depelim xy; solve_discr; t'. *)
-(*   - depelim xy; solve_discr. t'. *)
-
-(* eapply eq_universe_refl. *)
-(*   Set Typeclasses Debug Verbosity 2. *)
-(*   Fail typeclasses eauto. *)
-
-
-
-(* (*   induction xy; intros; auto. *) *)
-
-
-(* (*   eapply red_alt in *) *)
-(* (* xy. *) *)
-(* (*   eapply clos_rt_rt1n_iff in xy. *) *)
-(* (*   induction xy. intros. reflexivity. *) *)
-(* (*   intros zx. *) *)
-
-Lemma confluence_upto_leq `{cf : checker_flags} {Σ : global_env_ext} {Γ x y z} :
-  wf Σ ->
-  red Σ Γ x z -> red Σ Γ y z -> leq_term Σ x y -> eq_term Σ x y.
-Proof.
-  intros wfΣ xz.
-  eapply red_alt in xz.
-  eapply clos_rt_rt1n_iff in xz.
-  induction xz in y |- *.
-  intros yx xy.
-  eapply leq_term_antisym. auto.
-  induction xy; constructor; auto. eapply All2_sym; eauto. tc.
-  depelim yx. admit.
-Abort.
-
-(*
-
-   t   <=   u    <=   t           t0 <= t1 /\ t0 -> t' /\ t1 -> t' -> t0 = t1
-   |        |         |
-   |        |         |
-   v        v         v
-   t0  <=   u'  <=   t1
-    \               /
-     \            /
-      \          /
-       \        /
-        v      v
-           t'
-
-
-   t   <=   u    <=   t
-   |        |         |
-   |        |         |
-   v        v         v
-   t0  <=   u0  <=   t1
-    \      |         /
-     \     |       /
-      \  <=U->    /
-       \   |    /
-        v  v   v
-           t'
-
-
-*)
-
-Lemma leq_term_trans_sandwich `{cf : checker_flags} {Σ : global_env_ext} {t u u' v} :
-  wf Σ ->
-  leq_term Σ t u -> leq_term Σ u v ->
-  leq_term Σ v u' -> leq_term Σ u' t ->
-  eq_term Σ t v * (eq_term Σ u u' * eq_term Σ t u).
-Proof.
-  intros. assert (eq_term Σ t v).
-  eapply leq_term_antisym.
-  now transitivity u.
-  now transitivity u'.
-  split; auto. assert (eq_term Σ u u').
-  apply leq_term_antisym.
-  now transitivity v.
-  now transitivity t.
-  split; auto.
-  apply leq_term_antisym. auto.
-  transitivity v. auto. now transitivity u'.
-Qed.
-
-Lemma conv_alt_trans `{cf : checker_flags} {Σ : global_env_ext} {Γ t u v} :
-  wf Σ ->
-  Σ ;;; Γ |- t == u ->
-  Σ ;;; Γ |- u == v ->
-  Σ ;;; Γ |- t == v.
-Proof.
-  intros wfΣ X0 X1.
-  eapply conv_alt_red in X0 as [t' [u' [[tt' uu'] eq]]].
-  eapply conv_alt_red in X1 as [u'' [v' [[uu'' vv'] eq']]].
-  eapply conv_alt_red.
-  destruct (red_confluence wfΣ uu' uu'') as [u'nf [ul ur]].
-  eapply red_eq_term_upto_univ_r in ul as [tnf [redtnf ?]]. 10:eapply eq. all:tc. 2:trivial.
-  eapply red_eq_term_upto_univ_l in ur as [unf [redunf ?]]. 9:eapply eq'. all:tc. 2:trivial.
-  exists tnf, unf.
-  intuition auto.
-  now transitivity t'.
-  now transitivity v'.
-  now transitivity u'nf.
-Qed.
-
-Lemma cumul_trans_red_conv `{cf : checker_flags} {Σ : global_env_ext} {Γ t u} : wf Σ ->
-  Σ ;;; Γ |- t <= u -> Σ ;;; Γ |- u <= t -> Σ ;;; Γ |- t == u.
-Proof.
-  move=> wfΣ tu ut.
-  eapply cumul_trans_red_leqterm in ut; eauto.
-  destruct ut as [t0 [u0 [t1 [[[[tt0 t0u0] uu0] u0t1] tt1]]]].
-  (* eapply cumul_trans_red_leqterm in tu; eauto. *)
-  (* destruct tu as [u1 [t2 [u2 [[[[tt0' t0u0'] uu0'] u0t1'] tt1']]]]. *)
-  destruct (red_confluence wfΣ tt0 tt1) as [t' [t0t' t1t']].
-  eapply red_eq_term_upto_univ_lr in uu0 as [u0' [redu0' ?]].
-Admitted.
-
-  (* 10:eapply *)
-
-
-  (* eapply red_eq_term_upto_univ_r in u0t1 as [u0' [redu0' ?]]. *)
-  (* 10:eapply t1t'. all:tc. 2:apply eq_universe_leq_universe. *)
-  (* change (leq_term Σ u0' t') in e. *)
-  (* eapply red_eq_term_upto_univ_l in t0u0 as [u0'' [redu0'' ?]]. *)
-  (* 9:eapply t0t'. all:tc. 2:apply eq_universe_leq_universe. *)
-  (* change (leq_term Σ t' u0'') in e0. *)
-  (* apply conv_alt_red. *)
-  (* destruct (red_confluence wfΣ redu0' redu0'') as [u0nf [? ?]]. *)
-
-
-(*
-
-   t  <=  u
-   |      |
-   |      |
-   v      v
-   t' =>  u'
-
-*)
-
-
-
-Corollary confluence {cf : checker_flags} {Σ : global_env_ext} Γ Δ Δ' t u t' u' :
-  wf Σ ->
-  leq_term Σ t t' ->
-  pred1 Σ Γ Δ t t' ->
-  pred1 Σ Γ Δ' u u' ->
-  pred1 Σ Δ (rho_ctx Σ Γ) t' (rho Σ (rho_ctx Σ Γ) t) *
-  pred1 Σ Δ' (rho_ctx Σ Γ) u' (rho Σ (rho_ctx Σ Γ) u) *
-  leq_term Σ (rho Σ (rho_ctx Σ Γ) t) (rho Σ (rho_ctx Σ Γ) u).
-Proof.
-  intros wfΣ **.
-  split. eapply triangle in X0. eapply triangle in X. all:eauto.
-  induction H.
-Abort.
-
-(* Lemma fill_le' `{cf : checker_flags} {Σ : global_env_ext} {Γ t t' u u'} : *)
-(*   wf Σ -> *)
-(*   leq_term Σ t u -> red Σ Γ t t' -> red Σ Γ u u' -> (leq_term Σ t' u' + (leq_term Σ u' t' -> False)). *)
-(* Proof. *)
-(*   intros wfΣ tu tt' uu'. *)
-
-
-(*   pose proof tu as tu2. *)
-(*   eapply red_eq_term_upto_univ_r in uu'. 9:eapply tu2. all:tc. 2:eapply eq_universe_leq_universe. *)
-(*   destruct uu' as [t'' [t't'' t''unf]]. *)
-(*   assert (leq_term *)
-(*   intros. *)
-
-(*   exists t'', unf. intuition auto. *)
-(* Qed. *)
-
-
-(*   destruct (fill_le wfΣ u0t1 c t1t') as [u0'' [t'' [[u0'u0'' t't''] lequ0t'']]]. *)
-
-
-(*   destruct (commutes_horizontal_red_leq (Σ:=Σ) (Γ := Γ) (x:=u0) (y:=t')) as [u0'' [? ?]]. *)
-(*   exists t1. auto. *)
-
-(*   Lemma leq_term_gen_antisym {cf : checker_flags} φ x y y' : *)
-(*     leq_term φ x y -> leq_term φ y' x -> (eq_term φ x y * eq_term φ y' x). *)
-(*   Proof. *)
-(*   Admitted. *)
-
-(*   assert(red_leq Σ Γ u0 t'). *)
-(*   { transitivity t0. eapply leq_red_leq. *)
-
-
-
-(*   destruct (red_confluence wfΣ uu0 uu1) as [u' [? ?]]. *)
-(*   destruct (fill_le wfΣ leqt0u0 r r1) as [t'' [u0'' [[? ?] leqt''u0'']]]. *)
-(*   destruct (fill_le wfΣ lequ1t1 r2 r0) as [u1' [t1'' [[? ?] lequ1't1'']]]. *)
-
-(*
-
-   t   <=   u    <=   t
-   |        |         |
-   |        |         |
-   v        v         v
-   t0  <= u0 u1 <=   t1
-    \ \   \ /       /
-     \ \   u       /
-      \ v         /
-       \ x       /
-        v Λ     v
-            t'
-*)
-
-Require Import PCUICClosed.
-
-
-Section ContextConversion.
-  Context {cf : checker_flags}.
-  Context (Σ : global_env_ext).
-  Context (wfΣ : wf Σ).
-
-Inductive context_relation (P : context -> context -> context_decl -> context_decl -> Type)
-          : forall (Γ Γ' : context), Type :=
-| ctx_rel_nil : context_relation P nil nil
-| ctx_rel_vass na na' T U Γ Γ' :
-    context_relation P Γ Γ' ->
-    P Γ Γ' (vass na T) (vass na' U) ->
-    context_relation P (vass na T :: Γ) (vass na' U :: Γ')
-| ctx_rel_def na na' t T u U Γ Γ' :
-    context_relation P Γ Γ' ->
-    P Γ Γ' (vdef na t T) (vdef na' u U) ->
-    context_relation P (vdef na t T :: Γ) (vdef na' u U :: Γ').
-Derive Signature for context_relation.
-Arguments context_relation P Γ Γ' : clear implicits.
-
-Lemma context_relation_nth {P n Γ Γ' d} :
-  context_relation P Γ Γ' -> nth_error Γ n = Some d ->
-  { d' & ((nth_error Γ' n = Some d') *
-          let Γs := skipn (S n) Γ in
-          let Γs' := skipn (S n) Γ' in
-          context_relation P Γs Γs' *
-          P Γs Γs' d d')%type }.
-Proof.
-  induction n in Γ, Γ', d |- *; destruct Γ; intros Hrel H; noconf H.
-  - depelim Hrel.
-    simpl. eexists; intuition eauto.
-    eexists; intuition eauto.
-  - depelim Hrel.
-    destruct (IHn _ _ _ Hrel H).
-    cbn -[skipn] in *.
-    eexists; intuition eauto.
-
-    destruct (IHn _ _ _ Hrel H).
-    eexists; intuition eauto.
-Qed.
-
-  Inductive conv_decls Γ Γ' : forall (x y : context_decl), Type :=
-  | conv_vass na na' T T' :
-      isType Σ Γ' T' ->
-      Σ ;;; Γ |- T = T' ->
-      conv_decls Γ Γ' (vass na T) (vass na' T')
-
-  | conv_vdef_type na na' b T T' :
-      isType Σ Γ' T' ->
-      Σ ;;; Γ |- T = T' ->
-      conv_decls Γ Γ' (vdef na b T) (vdef na' b T')
-
-  | conv_vdef_body na na' b b' T T' :
-      isType Σ Γ' T' ->
-      Σ ;;; Γ' |- b' : T' ->
-      Σ ;;; Γ |- b = b' ->
-      Σ ;;; Γ |- T = T' ->
-      conv_decls Γ Γ' (vdef na b T) (vdef na' b' T').
-
-  Notation conv_context Γ Γ' := (context_relation conv_decls Γ Γ').
-End ContextConversion. (* Copied from SR *)
-
-Notation conv_context Σ Γ Γ' := (context_relation (conv_decls Σ) Γ Γ').
 Lemma cumul_Sort_inv {cf:checker_flags} Σ Γ s s' :
   Σ ;;; Γ |- tSort s <= tSort s' -> leq_universe (global_ext_constraints Σ) s s'.
 Proof.
@@ -1594,8 +92,8 @@ Lemma cumul_Prod_Sort_inv {cf:checker_flags} Σ Γ s na dom codom :
 Proof.
   intros H; depind H; auto.
   - now inversion l.
-  - depelim r. solve_discr. eapply IHcumul. reflexivity.
-    eapply IHcumul. reflexivity.
+  - depelim r. solve_discr. eapply IHcumul; reflexivity.
+    eapply IHcumul; reflexivity.
   - depelim r. solve_discr.
 Qed.
 
@@ -1604,18 +102,26 @@ Lemma cumul_Prod_Prod_inv {cf:checker_flags} (Σ : global_env_ext) Γ na na' dom
    ((Σ ;;; Γ |- dom = dom') * (Σ ;;; Γ ,, vass na' dom' |- codom <= codom'))%type.
 Proof.
   intros wfΣ H; depind H; auto.
-  - inv l. split; auto. admit. admit.
+  - inv l. split; auto. split; constructor; auto. now eapply eq_term_leq_term.
+    now eapply eq_term_leq_term, eq_term_sym.
+    constructor. eapply H0.
   - depelim r. solve_discr.
     destruct (IHcumul na na' N1 _ _ _ wfΣ eq_refl).
-    split; auto. admit.
+    split; auto. eapply conv_trans with N1=> //. now eapply red_conv, red1_red.
     destruct (IHcumul na na' _ _ N2 _ wfΣ eq_refl).
-    split; auto. eapply cumul_trans. auto. 2:eauto. eapply red_cumul.
-    admit.
+    split; auto. eapply cumul_trans. auto. 2:eauto.
+    eapply red1_red in r.
+    admit. (* Conversion of reduction for assumption context *)
   - depelim r. solve_discr.
     destruct (IHcumul na na' _ _ _ _ wfΣ eq_refl).
-    split; auto. admit. admit.
+    split; auto. eapply conv_trans with N1 => //. eapply conv_sym => //.
+    now eapply red_conv, red1_red.
+    eapply cumul_red_ctx_inv. auto. eauto. constructor. eapply All2_local_env_red_refl. red.
+    now eapply red1_red.
     destruct (IHcumul na na' _ _ _ _ wfΣ eq_refl).
-    split; auto. admit.
+    split; auto.
+    eapply cumul_trans with N2; auto.
+    eapply red1_red, red_conv in r. apply r.
 Admitted.
 
 Lemma assumption_context_app Γ Γ' :
@@ -1640,7 +146,7 @@ Proof.
   - eapply cumul_Sort_inv in X. split; constructor; auto.
   - destruct x as [na [b|] ty]. elimtype False.
     apply assumption_context_app in H0.
-    destruct H0. depelim a0. hnf in H0; depelim H0.
+    destruct H0. inv a0.
     rewrite it_mkProd_or_LetIn_app in X.
     apply assumption_context_app in H0 as [H0 _].
     specialize (IHctx' H0).
@@ -1664,90 +170,55 @@ Proof.
     intuition auto.
 Admitted.
 
-
-  Lemma conv_context_red_context {cf : checker_flags} (Σ : global_env_ext) Γ Γ' :
-    conv_context Σ Γ Γ' ->
-    ∑ Δ Δ', @red_ctx Σ Γ Δ * @red_ctx Σ Γ' Δ' * eq_context_upto (eq_universe (global_ext_constraints Σ)) Δ Δ'.
-  Proof.
-  Admitted.
-
-Lemma cumul_antisym `{cf : checker_flags} {Σ : global_env_ext} {Γ T U} :
-  wf Σ ->
-  isWfArity typing Σ [] T ->
-  isWfArity typing Σ [] U ->
-  Σ ;;; Γ |- T <= U -> Σ ;;; Γ |- U <= T -> Σ ;;; Γ |- T == U.
+(** Injectivity of products, the essential property of cumulativity needed for subject reduction. *)
+Lemma cumul_Prod_inv {cf:checker_flags} Σ Γ na na' A B A' B' :
+  wf Σ.1 -> wf_local Σ Γ ->
+  Σ ;;; Γ |- tProd na A B <= tProd na' A' B' ->
+   ((Σ ;;; Γ |- A == A') * (Σ ;;; Γ ,, vass na' A' |- B <= B'))%type.
 Proof.
-  move=> wfΣ tu ut.
-  red in tu, ut.
-  destruct tu as [ctx [s [Teq wf]]].
-  destruct ut as [ctx' [s' [Teq' wf']]].
-  generalize (destArity_spec [] T). rewrite Teq.
-  simpl. intros ->.
-  generalize (destArity_spec [] U). rewrite Teq'.
-  simpl. intros ->.
-  clear Teq Teq'.
-  intros.
+  intros wfΣ wfΓ H; depind H.
+  - depelim l.
+    split; auto.
+    now constructor.
+    now constructor.
 
-  Lemma cumul_smash_context {cf : checker_flags} Σ Γ ctx ctx' s s' :
-    Σ;;; Γ |- it_mkProd_or_LetIn ctx (tSort s) <= it_mkProd_or_LetIn ctx' (tSort s') <~>
-    Σ;;; Γ |- it_mkProd_or_LetIn (smash_context [] ctx) (tSort s) <=
-              it_mkProd_or_LetIn (smash_context [] ctx') (tSort s').
-  Proof.
-    revert ctx' s s'.
-    induction ctx; intros. simpl.
-  Admitted.
-    (* destruct ctx' as [|[na [b|] ty] ctx] using rev_ind. simpl. *)
-    (* split; auto. simpl. *)
-    (* rewrite it_mkProd_or_LetIn_app /= /mkProd_or_LetIn /=. *)
-    (* simpl in IHctx'. split; intros. *)
-    (* Lemma smash_context_app Γ ctx ctx' : *)
-    (*   smash_context Γ (ctx ++ ctx')%list = *)
-    (*   smash_context (smash_context Γ ctx') ctx. *)
-    (* Proof. *)
-    (*   induction ctx in Γ, ctx' |- *; simpl; auto. *)
-    (*   destruct a as [na [b|] ty]; auto. rewrite IHctx. simpl. *)
-    (*   f_equal. *)
-    (*   Lemma smash_context_subst s n Γ Γ' : *)
-    (*     smash_context (subst_context s n Γ) Γ' = subst_context s n (smash_context Γ Γ'). *)
-    (*   Proof. *)
-    (*     revert s n Γ'. *)
-    (*     induction Γ as [|[na [b|] ty]]; simpl; intros; auto. *)
-    (*     rewrite {1}/subst_context /fold_context /=. simpl. *)
-    (*     rewrite IHΓ'. rewrite -IHΓ'. *)
+  - depelim r. solve_discr.
+    specialize (IHcumul _ _ _ _ _ _ wfΣ wfΓ eq_refl).
+    intuition auto.
+    econstructor 2; eauto.
 
-    (* split; intros. *)
-    (* simpl in X. *)
+    specialize (IHcumul _ _ _ _ _ _ wfΣ wfΓ eq_refl).
+    intuition auto. apply cumul_trans with N2. auto.
+    eapply cumul_conv_ctx; eauto.
 
-  eapply cumul_smash_context in X.
-  eapply cumul_smash_context in X0.
+    econstructor 2. eauto. constructor. auto. constructor. now apply conv_ctx_refl.
+    constructor; auto.
+    auto.
 
-  Lemma assumption_context_smash_context Γ Γ' :
-    assumption_context Γ ->
-    assumption_context (smash_context Γ Γ').
-  Admitted.
-  have assctx := (@assumption_context_smash_context [] ctx assumption_context_nil).
-  have assctx' := (@assumption_context_smash_context [] ctx' assumption_context_nil).
-  eapply conv_alt_red.
-  eapply it_mkProd_or_LetIn_ass_inv in X; auto.
-  eapply it_mkProd_or_LetIn_ass_inv in X0; auto.
-  intuition auto.
-  destruct (conv_context_red_context a) as [Δ [Δ' [[redΔ redΔ'] ?]]].
-  exists (it_mkProd_or_LetIn Δ (tSort s)), (it_mkProd_or_LetIn Δ' (tSort s')).
-  intuition auto.
-  transitivity (it_mkProd_or_LetIn (smash_context [] ctx) (tSort s)).
-  admit. admit.
-  admit.
-  (* Need an eq_term upto contexts *)
-  admit.
-Admitted.
+  - depelim r. solve_discr.
+    specialize (IHcumul _ _ _ _ _ _ wfΣ wfΓ eq_refl).
+    intuition auto. econstructor 3. 2:eauto. auto.
+    eapply cumul_conv_ctx in b. eauto. auto. constructor. eapply conv_ctx_refl. auto.
+    constructor. eapply conv_alt_sym; auto.
 
-Existing Class wf.
+    specialize (IHcumul _ _ _ _ _ _ wfΣ wfΓ eq_refl).
+    intuition auto. apply cumul_trans with N2. auto. auto.
+    eapply cumul_red_r; eauto.
+Qed.
 
-Lemma cumul_conv_alt `{cf : checker_flags} {Σ : global_env_ext} {wfΣ : wf Σ} {Γ t u} :
-  Σ ;;; Γ |- t <= u -> Σ ;;; Γ |- u <= t -> Σ ;;; Γ |- t == u.
+Lemma tProd_it_mkProd_or_LetIn na A B ctx s :
+  tProd na A B = it_mkProd_or_LetIn ctx (tSort s) ->
+  { ctx' & ctx = (ctx' ++ [vass na A])%list /\
+           destArity [] B = Some (ctx', s) }.
 Proof.
-  intros l r.
-Admitted.
+  intros. exists (removelast ctx).
+  revert na A B s H.
+  induction ctx using rev_ind; intros; noconf H.
+  rewrite it_mkProd_or_LetIn_app in H. simpl in H.
+  destruct x as [na' [b'|] ty']; noconf H; simpl in *.
+  rewrite removelast_app. congruence. simpl. rewrite app_nil_r. intuition auto.
+  rewrite destArity_it_mkProd_or_LetIn. simpl. now rewrite app_context_nil_l.
+Qed.
 
 Section Inversions.
   Context {cf : checker_flags}.
@@ -1763,11 +234,11 @@ Section Inversions.
   Qed.
 
   Lemma cumul_App_r {Γ f u v} :
-    Σ ;;; Γ |- u = v ->
+    Σ ;;; Γ |- u == v ->
     Σ ;;; Γ |- tApp f u <= tApp f v.
   Proof.
     intros h.
-    apply conv_conv_alt in h => //. induction h.
+    induction h.
     - eapply cumul_refl. constructor.
       + apply leq_term_refl.
       + assumption.
@@ -1778,12 +249,11 @@ Section Inversions.
   Qed.
 
   Lemma conv_App_r {Γ f x y} :
-    Σ ;;; Γ |- x = y ->
-    Σ ;;; Γ |- tApp f x = tApp f y.
+    Σ ;;; Γ |- x == y ->
+    Σ ;;; Γ |- tApp f x == tApp f y.
   Proof.
     intros h.
-    eapply conv_conv_alt => //.
-    apply conv_conv_alt in h => //. induction h.
+    induction h.
     - constructor. constructor.
       + apply eq_term_refl.
       + assumption.
@@ -1795,12 +265,11 @@ Section Inversions.
 
   Lemma conv_Prod_l:
     forall {Γ na na' A1 A2 B},
-      Σ ;;; Γ |- A1 = A2 ->
-                 Σ ;;; Γ |- tProd na A1 B = tProd na' A2 B.
+      Σ ;;; Γ |- A1 == A2 ->
+      Σ ;;; Γ |- tProd na A1 B == tProd na' A2 B.
   Proof.
     intros Γ na na' A1 A2 B h.
-    eapply conv_conv_alt. tc.
-    apply conv_conv_alt in h. induction h.
+    induction h.
     - constructor. constructor.
       + assumption.
       + apply eq_term_refl.
@@ -1812,12 +281,11 @@ Section Inversions.
 
   Lemma conv_Prod_r  :
     forall {Γ na A B1 B2},
-      Σ ;;; Γ ,, vass na A |- B1 = B2 ->
-                              Σ ;;; Γ |- tProd na A B1 = tProd na A B2.
+      Σ ;;; Γ ,, vass na A |- B1 == B2 ->
+      Σ ;;; Γ |- tProd na A B1 == tProd na A B2.
   Proof.
     intros Γ na A B1 B2 h.
-    eapply conv_conv_alt.
-    apply conv_conv_alt in h. induction h.
+    induction h.
     - constructor. constructor.
       + apply eq_term_refl.
       + assumption.
@@ -1830,7 +298,7 @@ Section Inversions.
   Lemma cumul_Prod_r :
     forall {Γ na A B1 B2},
       Σ ;;; Γ ,, vass na A |- B1 <= B2 ->
-                              Σ ;;; Γ |- tProd na A B1 <= tProd na A B2.
+      Σ ;;; Γ |- tProd na A B1 <= tProd na A B2.
   Proof.
     intros Γ na A B1 B2 h.
     induction h.
@@ -1845,11 +313,10 @@ Section Inversions.
 
   Lemma conv_cumul_l :
     forall Γ u v,
-      Σ ;;; Γ |- u = v ->
-                 Σ ;;; Γ |- u <= v.
+      Σ ;;; Γ |- u == v ->
+      Σ ;;; Γ |- u <= v.
   Proof.
-    intros Γ u v [? ?].
-    assumption.
+    intros Γ u v h. now eapply conv_alt_cumul.
   Qed.
 
   Lemma conv_refl' :
@@ -1858,29 +325,20 @@ Section Inversions.
   Proof.
     intros leq Γ t.
     destruct leq.
-    - cbn. constructor. apply conv_refl'.
+    - cbn. constructor. apply conv_alt_refl. reflexivity.
     - cbn. constructor. apply cumul_refl'.
-  Qed.
-
-  Lemma conv_sym :
-    forall Γ u v,
-      Σ ;;; Γ |- u = v ->
-                 Σ ;;; Γ |- v = u.
-  Proof.
-    intros Γ u v [h1 h2].
-    econstructor ; assumption.
   Qed.
 
   Lemma conv_conv :
     forall {Γ leq u v},
-      ∥ Σ ;;; Γ |- u = v ∥ ->
-                   conv leq Σ Γ u v.
+      ∥ Σ ;;; Γ |- u == v ∥ ->
+      conv leq Σ Γ u v.
   Proof.
     intros Γ leq u v h.
     destruct leq.
     - assumption.
-    - destruct h as [[h1 h2]]. cbn.
-      constructor. assumption.
+    - destruct h. cbn.
+      constructor. now eapply conv_alt_cumul.
   Qed.
 
   Lemma eq_term_conv :
@@ -1898,16 +356,6 @@ Section Inversions.
       assumption.
   Qed.
 
-  Lemma conv_trans :
-    forall Γ u v w,
-      Σ ;;; Γ |- u = v ->
-                 Σ ;;; Γ |- v = w ->
-                            Σ ;;; Γ |- u = w.
-  Proof.
-    intros Γ u v w h1 h2.
-    destruct h1, h2. constructor ; eapply cumul_trans ; eassumption.
-  Qed.
-
   Lemma conv_trans' :
     forall leq Γ u v w,
       conv leq Σ Γ u v ->
@@ -1917,7 +365,7 @@ Section Inversions.
     intros leq Γ u v w h1 h2.
     destruct leq.
     - cbn in *. destruct h1, h2. constructor.
-      eapply conv_trans ; eassumption.
+      eapply conv_alt_trans ; eassumption.
     - cbn in *. destruct h1, h2. constructor. eapply cumul_trans ; eassumption.
   Qed.
 
@@ -1931,13 +379,8 @@ Section Inversions.
     - apply conv_refl'.
     - eapply conv_trans' ; try eassumption.
       destruct leq.
-      + simpl. constructor. constructor.
-        * eapply cumul_red_l.
-          -- eassumption.
-          -- eapply cumul_refl'.
-        * eapply cumul_red_r.
-          -- eapply cumul_refl'.
-          -- assumption.
+      + simpl. destruct IHh. constructor.
+        eapply conv_alt_red_l; eauto.
       + simpl. constructor.
         eapply cumul_red_l.
         * eassumption.
@@ -1954,13 +397,8 @@ Section Inversions.
     - apply conv_refl'.
     - eapply conv_trans' ; try eassumption.
       destruct leq.
-      + simpl. constructor. constructor.
-        * eapply cumul_red_r.
-          -- eapply cumul_refl'.
-          -- assumption.
-        * eapply cumul_red_l.
-          -- eassumption.
-          -- eapply cumul_refl'.
+      + simpl. destruct IHh. constructor.
+        eapply conv_alt_red_r; eauto.
       + simpl. constructor.
         eapply cumul_red_r.
         * eapply cumul_refl'.
@@ -1969,13 +407,13 @@ Section Inversions.
 
   Lemma conv_Prod :
     forall leq Γ na A1 A2 B1 B2,
-      Σ ;;; Γ |- A1 = A2 ->
-                 conv leq Σ (Γ,, vass na A1) B1 B2 ->
-                 conv leq Σ Γ (tProd na A1 B1) (tProd na A2 B2).
+      Σ ;;; Γ |- A1 == A2 ->
+      conv leq Σ (Γ,, vass na A1) B1 B2 ->
+      conv leq Σ Γ (tProd na A1 B1) (tProd na A2 B2).
   Proof.
     intros [] Γ na A1 A2 B1 B2 h1 h2.
     - simpl in *. destruct h2 as [h2]. constructor.
-      eapply conv_trans.
+      eapply conv_alt_trans => //.
       + eapply conv_Prod_r. eassumption.
       + eapply conv_Prod_l. eassumption.
     - simpl in *. destruct h2 as [h2]. constructor.
@@ -1986,17 +424,17 @@ Section Inversions.
 
   Lemma cumul_Case_c :
     forall Γ indn p brs u v,
-      Σ ;;; Γ |- u = v ->
-                 Σ ;;; Γ |- tCase indn p u brs <= tCase indn p v brs.
+      Σ ;;; Γ |- u == v ->
+      Σ ;;; Γ |- tCase indn p u brs <= tCase indn p v brs.
   Proof.
     intros Γ [ind n] p brs u v h.
-    eapply conv_conv_alt in h.
     induction h.
     - constructor. constructor.
       + eapply eq_term_refl.
       + assumption.
       + eapply All2_same.
         intros. split ; eauto.
+        reflexivity.
     - eapply cumul_red_l ; eauto.
       constructor. assumption.
     - eapply cumul_red_r ; eauto.
@@ -2005,11 +443,10 @@ Section Inversions.
 
   Lemma cumul_Proj_c :
     forall Γ p u v,
-      Σ ;;; Γ |- u = v ->
-                 Σ ;;; Γ |- tProj p u <= tProj p v.
+      Σ ;;; Γ |- u == v ->
+      Σ ;;; Γ |- tProj p u <= tProj p v.
   Proof.
     intros Γ p u v h.
-    eapply conv_conv_alt in h.
     induction h.
     - eapply cumul_refl. constructor. assumption.
     - eapply cumul_red_l ; try eassumption.
@@ -2020,12 +457,11 @@ Section Inversions.
 
   Lemma conv_App_l :
     forall {Γ f g x},
-      Σ ;;; Γ |- f = g ->
-                 Σ ;;; Γ |- tApp f x = tApp g x.
+      Σ ;;; Γ |- f == g ->
+      Σ ;;; Γ |- tApp f x == tApp g x.
   Proof.
     intros Γ f g x h.
-    eapply conv_conv_alt.
-    apply conv_conv_alt in h. induction h.
+    induction h.
     - constructor. constructor.
       + assumption.
       + apply eq_term_refl.
@@ -2037,18 +473,16 @@ Section Inversions.
 
   Lemma conv_Case_c :
     forall Γ indn p brs u v,
-      Σ ;;; Γ |- u = v ->
-                 Σ ;;; Γ |- tCase indn p u brs = tCase indn p v brs.
+      Σ ;;; Γ |- u == v ->
+      Σ ;;; Γ |- tCase indn p u brs == tCase indn p v brs.
   Proof.
     intros Γ [ind n] p brs u v h.
-    eapply conv_conv_alt in h.
-    apply conv_conv_alt.
     induction h.
     - constructor. constructor.
       + eapply eq_term_refl.
       + assumption.
       + eapply All2_same.
-        intros. split ; eauto.
+        intros. split ; eauto. reflexivity.
     - eapply conv_alt_red_l ; eauto.
       constructor. assumption.
     - eapply conv_alt_red_r ; eauto.
@@ -2057,12 +491,10 @@ Section Inversions.
 
   Lemma conv_Proj_c :
     forall Γ p u v,
-      Σ ;;; Γ |- u = v ->
-                 Σ ;;; Γ |- tProj p u = tProj p v.
+      Σ ;;; Γ |- u == v ->
+      Σ ;;; Γ |- tProj p u == tProj p v.
   Proof.
     intros Γ p u v h.
-    eapply conv_conv_alt in h.
-    apply conv_conv_alt.
     induction h.
     - eapply conv_alt_refl. constructor. assumption.
     - eapply conv_alt_red_l ; try eassumption.
@@ -2073,12 +505,10 @@ Section Inversions.
 
   Lemma conv_Lambda_l :
     forall Γ na A b na' A',
-      Σ ;;; Γ |- A = A' ->
-                 Σ ;;; Γ |- tLambda na A b = tLambda na' A' b.
+      Σ ;;; Γ |- A == A' ->
+      Σ ;;; Γ |- tLambda na A b == tLambda na' A' b.
   Proof.
     intros Γ na A b na' A' h.
-    eapply conv_conv_alt in h.
-    apply conv_conv_alt.
     induction h.
     - eapply conv_alt_refl. constructor.
       + assumption.
@@ -2091,12 +521,10 @@ Section Inversions.
 
   Lemma conv_Lambda_r :
     forall Γ na A b b',
-      Σ ;;; Γ,, vass na A |- b = b' ->
-                             Σ ;;; Γ |- tLambda na A b = tLambda na A b'.
+      Σ ;;; Γ,, vass na A |- b == b' ->
+      Σ ;;; Γ |- tLambda na A b == tLambda na A b'.
   Proof.
     intros Γ na A b b' h.
-    eapply conv_conv_alt in h.
-    apply conv_conv_alt.
     induction h.
     - eapply conv_alt_refl. constructor.
       + eapply eq_term_refl.
@@ -2110,7 +538,7 @@ Section Inversions.
   Lemma cumul_LetIn_bo :
     forall Γ na ty t u u',
       Σ ;;; Γ ,, vdef na ty t |- u <= u' ->
-                                 Σ ;;; Γ |- tLetIn na ty t u <= tLetIn na ty t u'.
+      Σ ;;; Γ |- tLetIn na ty t u <= tLetIn na ty t u'.
   Proof.
     intros Γ na ty t u u' h.
     induction h.
@@ -2126,7 +554,7 @@ Section Inversions.
   Lemma cumul_Lambda_r :
     forall Γ na A b b',
       Σ ;;; Γ,, vass na A |- b <= b' ->
-                             Σ ;;; Γ |- tLambda na A b <= tLambda na A b'.
+      Σ ;;; Γ |- tLambda na A b <= tLambda na A b'.
   Proof.
     intros Γ na A b b' h.
     induction h.
@@ -2142,7 +570,7 @@ Section Inversions.
   Lemma cumul_it_mkLambda_or_LetIn :
     forall Δ Γ u v,
       Σ ;;; (Δ ,,, Γ) |- u <= v ->
-                         Σ ;;; Δ |- it_mkLambda_or_LetIn Γ u <= it_mkLambda_or_LetIn Γ v.
+      Σ ;;; Δ |- it_mkLambda_or_LetIn Γ u <= it_mkLambda_or_LetIn Γ v.
   Proof.
     intros Δ Γ u v h. revert Δ u v h.
     induction Γ as [| [na [b|] A] Γ ih ] ; intros Δ u v h.
@@ -2156,7 +584,7 @@ Section Inversions.
   Lemma cumul_it_mkProd_or_LetIn :
     forall Δ Γ B B',
       Σ ;;; (Δ ,,, Γ) |- B <= B' ->
-                         Σ ;;; Δ |- it_mkProd_or_LetIn Γ B <= it_mkProd_or_LetIn Γ B'.
+      Σ ;;; Δ |- it_mkProd_or_LetIn Γ B <= it_mkProd_or_LetIn Γ B'.
   Proof.
     intros Δ Γ B B' h.
     induction Γ as [| [na [b|] A] Γ ih ] in Δ, B, B', h |- *.
